08ByteCode/CodeFlattening.thy
@@ -15,8 +15,8 @@ fun flatten_code' :: "nat \<Rightarrow> code\<^sub>e list \<Rightarrow> code\<^s
 | "flatten_code' p (Lookup\<^sub>e x y # \<C>) = flatten_code' p \<C> @ [Lookup\<^sub>b x y]"
 | "flatten_code' p (PushCon\<^sub>e n # \<C>) = flatten_code' p \<C> @ [PushCon\<^sub>b n]"
 | "flatten_code' p (PushLam\<^sub>e \<C>' n # \<C>) = (
-    let \<C>\<^sub>b' = flatten_code' p \<C>'
-    in \<C>\<^sub>b' @ flatten_code' (p + length \<C>\<^sub>b') \<C> @ [PushLam\<^sub>b (p + length \<C>\<^sub>b') n])"
+    let \<C>\<^sub>b' = flatten_code' p \<C>' @ [Alloc\<^sub>b n]
+    in \<C>\<^sub>b' @ flatten_code' (p + length \<C>\<^sub>b') \<C> @ [PushLam\<^sub>b (p + length \<C>\<^sub>b')])"
 | "flatten_code' p (Apply\<^sub>e # \<C>) = flatten_code' p \<C> @ [Apply\<^sub>b]"
 | "flatten_code' p (PushEnv\<^sub>e # \<C>) = flatten_code' p \<C> @ [PushEnv\<^sub>b]"
 | "flatten_code' p (Return\<^sub>e # \<C>) = flatten_code' p \<C> @ [Return\<^sub>b]"
@@ -46,7 +46,7 @@ primrec code_size :: "code\<^sub>e \<Rightarrow> nat"
     and code_list_size :: "code\<^sub>e list \<Rightarrow> nat" where
   "code_size (Lookup\<^sub>e x y) = 1"
 | "code_size (PushCon\<^sub>e n) = 1"
-| "code_size (PushLam\<^sub>e \<C> n) = Suc (code_list_size \<C>)"
+| "code_size (PushLam\<^sub>e \<C> n) = Suc (Suc (code_list_size \<C>))"
 | "code_size Apply\<^sub>e = 1"
 | "code_size PushEnv\<^sub>e = 1"
 | "code_size Return\<^sub>e = 1"
@@ -66,15 +66,13 @@ lemma code_size_nz [simp]: "0 < code_size op"
 lemma code_list_size_empty [simp]: "(code_list_size \<C> = 0) = (\<C> = [])"
   by (induction \<C>) simp_all
 
-lemma index_into_append [simp]: "pop_free \<C> \<Longrightarrow> 
+lemma index_into_append [simp]: "
     lookup (flatten_code' m \<C> @ \<C>') (code_list_size \<C> + n) = lookup \<C>' n"
   by (metis length_flatten' lookup_append_snd)
 
-lemma index_into_flatten [simp]: "pop_free \<C> \<Longrightarrow> 
-  lookup (flatten_code' n \<C> @ op # \<C>') (code_list_size \<C>) = Some op"
+lemma index_into_flatten [simp]: "lookup (flatten_code' n \<C> @ op # \<C>') (code_list_size \<C>) = Some op"
 proof -
-  assume "pop_free \<C>"
-  hence "lookup (flatten_code' n \<C> @ op # \<C>') (code_list_size \<C> + 0) = lookup (op # \<C>') 0" 
+  have "lookup (flatten_code' n \<C> @ op # \<C>') (code_list_size \<C> + 0) = lookup (op # \<C>') 0" 
     by (metis index_into_append)
   thus ?thesis by simp
 qed
@@ -88,13 +86,21 @@ code would be the same, of course, but rather than get bogged down in trying to 
 Note the importance for termination of each nested code pointer being less than the address of its 
 operation.\<close>
 
+primrec alloc_size :: "code\<^sub>b list \<Rightarrow> nat \<Rightarrow> nat" where
+  "alloc_size \<C> 0 = undefined"
+| "alloc_size \<C> (Suc p) = (case lookup \<C> p of
+      Some (Alloc\<^sub>b n) \<Rightarrow> n
+    | _ \<Rightarrow> undefined)"
+
 fun unflatten_code :: "code\<^sub>b list \<Rightarrow> nat \<Rightarrow> code\<^sub>e list" where
   "unflatten_code \<C> 0 = []"
 | "unflatten_code \<C> (Suc p) = (case lookup \<C> p of
       Some (Lookup\<^sub>b x y) \<Rightarrow> Lookup\<^sub>e x y # unflatten_code \<C> p
     | Some (PushCon\<^sub>b n) \<Rightarrow>  PushCon\<^sub>e n # unflatten_code \<C> p
-    | Some (PushLam\<^sub>b p' n) \<Rightarrow> (
-        if p' \<le> p then PushLam\<^sub>e (unflatten_code \<C> p') n # unflatten_code \<C> p else undefined) 
+    | Some (PushLam\<^sub>b p') \<Rightarrow> (
+        if p' \<le> p then PushLam\<^sub>e (unflatten_code \<C> p') (alloc_size \<C> p') # unflatten_code \<C> p 
+        else undefined) 
+    | Some (Alloc\<^sub>b n) \<Rightarrow> unflatten_code \<C> p
     | Some Apply\<^sub>b \<Rightarrow> Apply\<^sub>e # unflatten_code \<C> p
     | Some PushEnv\<^sub>b \<Rightarrow> PushEnv\<^sub>e # unflatten_code \<C> p
     | Some Return\<^sub>b \<Rightarrow> [Return\<^sub>e]
@@ -103,8 +109,8 @@ fun unflatten_code :: "code\<^sub>b list \<Rightarrow> nat \<Rightarrow> code\<^
 
 primrec unflatten_closure :: "code\<^sub>b list \<Rightarrow> closure\<^sub>b \<Rightarrow> closure\<^sub>e" where
   "unflatten_closure \<C> (Const\<^sub>b n) = Const\<^sub>e n"
-| "unflatten_closure \<C> (Lam\<^sub>b \<Delta> p n) = 
-    Lam\<^sub>e (map (map (unflatten_closure \<C>)) \<Delta>) (unflatten_code \<C> p) n"
+| "unflatten_closure \<C> (Lam\<^sub>b \<Delta> p) = 
+    Lam\<^sub>e (map (map (unflatten_closure \<C>)) \<Delta>) (unflatten_code \<C> p) (alloc_size \<C> p)"
 
 abbreviation unflatten_values :: "code\<^sub>b list \<Rightarrow> closure\<^sub>b list \<Rightarrow> closure\<^sub>e list" where
   "unflatten_values \<C> \<V> \<equiv> map (unflatten_closure \<C>) \<V>"
@@ -118,6 +124,9 @@ abbreviation unflatten_stack :: "code\<^sub>b list \<Rightarrow> (closure\<^sub>
 primrec unflatten_state :: "code\<^sub>b list \<Rightarrow> state\<^sub>b \<Rightarrow> state\<^sub>e" where
   "unflatten_state \<C> (S\<^sub>b \<V> s) = S\<^sub>e (unflatten_values \<C> \<V>) (unflatten_stack \<C> s)"
 
+lemma unflatten_alloc_front [simp]: "p \<le> length \<C> \<Longrightarrow> alloc_size (\<C> @ \<C>') p = alloc_size \<C> p"
+  by (induction p) simp_all
+
 lemma unflatten_front [simp]: "p \<le> length \<C> \<Longrightarrow> unflatten_code (\<C> @ \<C>') p = unflatten_code \<C> p"
   by (induction \<C> p rule: unflatten_code.induct) (simp_all split: option.splits code\<^sub>b.splits) 
 
@@ -125,22 +134,27 @@ lemma unflatten_flatten' [simp]: "properly_terminated\<^sub>e \<C> \<Longrightar
   unflatten_code (\<C>' @ flatten_code' (length \<C>') \<C> @ \<C>'') (length \<C>' + code_list_size \<C>) = \<C>"
 proof (induction "length \<C>'" \<C> arbitrary: \<C>' \<C>'' rule: flatten_code'.induct)
   case (4 \<C>\<^sub>2 n \<C>\<^sub>1)
-  let ?pc = "length \<C>' + code_list_size \<C>\<^sub>2"
-  let ?code' = "\<C>' @ flatten_code' (length \<C>') \<C>\<^sub>2 @ []"
-  let ?code = "?code' @ flatten_code' ?pc \<C>\<^sub>1 @ PushLam\<^sub>b ?pc n # \<C>''"
-  have X: "length \<C>' + length (flatten_code' (length \<C>') \<C>\<^sub>2) = length ?code'" by simp
+  let ?pc = "Suc (length \<C>' + code_list_size \<C>\<^sub>2)"
+  let ?code' = "\<C>' @ flatten_code' (length \<C>') \<C>\<^sub>2 @ [Alloc\<^sub>b n]"
+  let ?code = "?code' @ flatten_code' ?pc \<C>\<^sub>1 @ PushLam\<^sub>b ?pc # \<C>''"
+  have X: "length \<C>' + length (flatten_code' (length \<C>') \<C>\<^sub>2 @ [Alloc\<^sub>b n]) = length ?code'" by simp
   from 4 have "properly_terminated\<^sub>e \<C>\<^sub>1" by simp
   with 4 X have "unflatten_code (?code' @ flatten_code' (length ?code') \<C>\<^sub>1 @
-    PushLam\<^sub>b (length \<C>' + length (flatten_code' (length \<C>') \<C>\<^sub>2)) n # \<C>'')
+    PushLam\<^sub>b (Suc (length \<C>' + length (flatten_code' (length \<C>') \<C>\<^sub>2))) # \<C>'')
       (length ?code' + code_list_size \<C>\<^sub>1) = \<C>\<^sub>1" by blast
-  with 4 have "unflatten_code ?code (length \<C>' + code_list_size \<C>\<^sub>2 + code_list_size \<C>\<^sub>1) = \<C>\<^sub>1" by simp
-  hence X: "unflatten_code ?code (length \<C>' + (code_list_size \<C>\<^sub>2 + code_list_size \<C>\<^sub>1)) = \<C>\<^sub>1" 
-    by (metis add.assoc)
+  with 4 have X: "unflatten_code ?code (?pc + code_list_size \<C>\<^sub>1) = \<C>\<^sub>1" by simp
   from 4 have "properly_terminated\<^sub>e \<C>\<^sub>2" by simp
   with 4 have "unflatten_code ?code' (length \<C>' + code_list_size \<C>\<^sub>2) = \<C>\<^sub>2" by blast
+  hence "unflatten_code ?code' ?pc = \<C>\<^sub>2" by simp
   moreover from 4 have "?pc \<le> length ?code'" by simp
-  ultimately have Z: "unflatten_code ?code ?pc = \<C>\<^sub>2" by (metis unflatten_front)
-  with 4 X Z show ?case by simp
+  ultimately have Y: "unflatten_code ?code ?pc = \<C>\<^sub>2" by (metis unflatten_front)
+  have "lookup (Alloc\<^sub>b n # flatten_code' ?pc \<C>\<^sub>1 @ PushLam\<^sub>b ?pc # \<C>'') (Suc (code_list_size \<C>\<^sub>1)) =
+    Some (PushLam\<^sub>b (Suc (length \<C>' + code_list_size \<C>\<^sub>2)))" by simp
+  hence "lookup (\<C>' @ flatten_code' (length \<C>') \<C>\<^sub>2 @ Alloc\<^sub>b n # flatten_code' ?pc \<C>\<^sub>1 @ 
+    PushLam\<^sub>b ?pc # \<C>'') (length \<C>' + (code_list_size \<C>\<^sub>2 + Suc (code_list_size \<C>\<^sub>1))) =
+      Some (PushLam\<^sub>b (Suc (length \<C>' + code_list_size \<C>\<^sub>2)))"
+    by (metis lookup_append_snd index_into_append)
+  with X Y show ?case by (simp add: add.assoc)
 qed simp_all
 
 lemma unflatten_flatten [simp]: "properly_terminated\<^sub>e \<C> \<Longrightarrow> 
@@ -156,7 +170,7 @@ text \<open>We have noted already that all the pointers in the codebase should g
 addresses. We now define some predicates to assert this formally:\<close>
 
 fun orderly_op :: "nat \<Rightarrow> code\<^sub>b \<Rightarrow> bool" where
-  "orderly_op n (PushLam\<^sub>b p m) = (0 < p \<and> p \<le> n)"
+  "orderly_op n (PushLam\<^sub>b p) = (0 < p \<and> p \<le> n)"
 | "orderly_op n _ = True"
 
 primrec orderly_code :: "code\<^sub>b list \<Rightarrow> nat \<Rightarrow> bool" where
@@ -165,7 +179,7 @@ primrec orderly_code :: "code\<^sub>b list \<Rightarrow> nat \<Rightarrow> bool"
 
 primrec orderly_closure :: "nat \<Rightarrow> closure\<^sub>b \<Rightarrow> bool" where
   "orderly_closure n (Const\<^sub>b m) = True"
-| "orderly_closure n (Lam\<^sub>b \<Delta> p m) = (0 < p \<and> p \<le> n \<and> list_all (list_all (orderly_closure n)) \<Delta>)"
+| "orderly_closure n (Lam\<^sub>b \<Delta> p) = (0 < p \<and> p \<le> n \<and> list_all (list_all (orderly_closure n)) \<Delta>)"
 
 fun orderly_stack :: "(closure\<^sub>b list list \<times> nat) list \<Rightarrow> nat \<Rightarrow> bool" where
   "orderly_stack [] n = True"
@@ -174,11 +188,11 @@ fun orderly_stack :: "(closure\<^sub>b list list \<times> nat) list \<Rightarrow
     (p < n \<and> \<Delta> \<noteq> [] \<and> list_all (list_all (orderly_closure n)) \<Delta> \<and> orderly_stack s n)"
 
 primrec orderly_state :: "code\<^sub>b list \<Rightarrow> state\<^sub>b \<Rightarrow> bool" where
-  "orderly_state \<C> (S\<^sub>b \<V> s) = (orderly_code \<C> 0 \<and> properly_terminated\<^sub>b \<C> \<and> 
+  "orderly_state \<C> (S\<^sub>b \<V> s) = (orderly_code \<C> 0 \<and> properly_terminated\<^sub>b \<C> \<and> block_structured\<^sub>b \<C> \<and>
     orderly_stack s (length \<C>) \<and> list_all (orderly_closure (length \<C>)) \<V>)"
 
 lemma orderly_append [simp]: "orderly_code (\<C> @ \<C>') n = 
-    (orderly_code \<C> n \<and> orderly_code \<C>' (length \<C> + n))"
+      (orderly_code \<C> n \<and> orderly_code \<C>' (length \<C> + n))"
   by (induction \<C> arbitrary: n) simp_all
 
 lemma orderly_flatten' [simp]: "p \<le> n \<Longrightarrow> properly_terminated\<^sub>e \<C> \<Longrightarrow> 
@@ -204,18 +218,18 @@ proof -
   ultimately show ?thesis by simp
 qed
 
-lemma pushlam_ordered' [simp]: "lookup \<C> x = Some (PushLam\<^sub>b p m) \<Longrightarrow> orderly_code \<C> n \<Longrightarrow> 
+lemma pushlam_ordered' [simp]: "lookup \<C> x = Some (PushLam\<^sub>b p) \<Longrightarrow> orderly_code \<C> n \<Longrightarrow> 
     x < length \<C> \<Longrightarrow> 0 < p \<and> p \<le> length \<C> + n"
   by (induction \<C> x arbitrary: n rule: lookup.induct) fastforce+
 
-lemma pushlam_ordered [simp]: "lookup \<C> x = Some (PushLam\<^sub>b p n) \<Longrightarrow> orderly_code \<C> 0 \<Longrightarrow> 
+lemma pushlam_ordered [simp]: "lookup \<C> x = Some (PushLam\<^sub>b p) \<Longrightarrow> orderly_code \<C> 0 \<Longrightarrow> 
     x < length \<C> \<Longrightarrow> 0 < p \<and> p \<le> length \<C>"
   using pushlam_ordered' by fastforce
 
-lemma orderly_lam' [simp]: "lookup \<C> p = Some (PushLam\<^sub>b p' m) \<Longrightarrow> orderly_code \<C> n \<Longrightarrow> p' \<le> p + n"
+lemma orderly_lam' [simp]: "lookup \<C> p = Some (PushLam\<^sub>b p') \<Longrightarrow> orderly_code \<C> n \<Longrightarrow> p' \<le> p + n"
   by (induction \<C> p arbitrary: n rule: lookup.induct) fastforce+
 
-lemma orderly_lam [simp]: "lookup \<C> p = Some (PushLam\<^sub>b p' m) \<Longrightarrow> orderly_code \<C> 0 \<Longrightarrow> p' \<le> p"
+lemma orderly_lam [simp]: "lookup \<C> p = Some (PushLam\<^sub>b p') \<Longrightarrow> orderly_code \<C> 0 \<Longrightarrow> p' \<le> p"
   using orderly_lam' by fastforce
 
 text \<open>Evaluation preserves the property of being orderly:\<close>
@@ -236,11 +250,14 @@ next
     with ev\<^sub>b_pushlam show ?thesis by (cases cd) simp_all
   qed simp_all
 next
+  case (ev\<^sub>b_alloc \<C> pc n \<V> \<Delta> s)
+  thus ?case by (cases pc, cases \<C>) simp_all
+next
   case (ev\<^sub>b_apply cd pc v env' pc' vs env s)
   thus ?case by (cases pc', simp, cases pc, cases cd) simp_all
 next
   case (ev\<^sub>b_pushenv cd pc v vs env s)
-  then show ?case by (cases pc, cases cd) simp_all
+  thus ?case by (cases pc, cases cd) simp_all
 next
   case (ev\<^sub>b_jump cd pc v env' pc' vs env s)
   thus ?case by (cases pc') simp_all
@@ -270,18 +287,18 @@ next
     unflatten_stack \<C> s)" by simp
   thus ?case by simp
 next
-  case (ev\<^sub>b_pushlam \<C> p p' n \<V> \<Delta> s)
+  case (ev\<^sub>b_pushlam \<C> p p' \<V> \<Delta> s)
   moreover hence X: "p' \<le> p" by auto
   moreover have "iter (\<leadsto>\<^sub>e) (S\<^sub>e (unflatten_values \<C> \<V>) ((map (unflatten_values \<C>) \<Delta>, 
-    PushLam\<^sub>e (unflatten_code \<C> p') n # unflatten_code \<C> p) # unflatten_stack \<C> s))
-    (S\<^sub>e (Lam\<^sub>e (map (unflatten_values \<C>) \<Delta>) (unflatten_code \<C> p') n # unflatten_values \<C> \<V>) 
-    ((map (unflatten_values \<C>) \<Delta>, unflatten_code \<C> p) # unflatten_stack \<C> s))" 
+    PushLam\<^sub>e (unflatten_code \<C> p') (alloc_size \<C> p') # unflatten_code \<C> p) # unflatten_stack \<C> s))
+    (S\<^sub>e (Lam\<^sub>e (map (unflatten_values \<C>) \<Delta>) (unflatten_code \<C> p') (alloc_size \<C> p') # 
+    unflatten_values \<C> \<V>) ((map (unflatten_values \<C>) \<Delta>, unflatten_code \<C> p) # unflatten_stack \<C> s))" 
       by (metis ev\<^sub>e_pushlam iter_one)
   ultimately show ?case by simp
 next
-  case (ev\<^sub>b_apply \<C> p v \<Delta>' p' n \<V> \<Delta> s)
-  hence "S\<^sub>e (unflatten_closure \<C> v # Lam\<^sub>e (map (unflatten_values \<C>) \<Delta>') (unflatten_code \<C> p') n # 
-    unflatten_values \<C> \<V>) 
+  case (ev\<^sub>b_apply \<C> p v \<Delta>' p' \<V> \<Delta> s)
+  hence "S\<^sub>e (unflatten_closure \<C> v # Lam\<^sub>e (map (unflatten_values \<C>) \<Delta>') (unflatten_code \<C> p') 
+    (alloc_size \<C> p') # unflatten_values \<C> \<V>) 
     ((map (unflatten_values \<C>) \<Delta>, unflatten_code \<C> (Suc p)) # unflatten_stack \<C> s) \<leadsto>\<^sub>e
     S\<^sub>e (unflatten_values \<C> \<V>) (([unflatten_closure \<C> v] # map (unflatten_values \<C>) \<Delta>', 
     unflatten_code \<C> p') # (map (unflatten_values \<C>) \<Delta>, unflatten_code \<C> p) # unflatten_stack \<C> s)" 
@@ -301,138 +318,194 @@ next
     (S\<^sub>e (unflatten_values \<C> \<V>) (unflatten_stack \<C> s))" by (metis ev\<^sub>e_return iter_one)
   ultimately show ?case by simp
 next
-  case (ev\<^sub>b_jump \<C> p v \<Delta>' p' n \<V> \<Delta> s)
-  have "S\<^sub>e (unflatten_closure \<C> v # Lam\<^sub>e (map (unflatten_values \<C>) \<Delta>') (unflatten_code \<C> p') n # 
-    unflatten_values \<C> \<V>) ((map (unflatten_values \<C>) \<Delta>, [Jump\<^sub>e]) # unflatten_stack \<C> s) \<leadsto>\<^sub>e 
-    S\<^sub>e (unflatten_values \<C> \<V>) (([unflatten_closure \<C> v] # map (unflatten_values \<C>) \<Delta>', 
-    unflatten_code \<C> p') # unflatten_stack \<C> s)" by (metis ev\<^sub>e_jump)
-  with ev\<^sub>b_jump have "S\<^sub>e (unflatten_closure \<C> v # 
-    Lam\<^sub>e (map (unflatten_values \<C>) \<Delta>') (unflatten_code \<C> p') n # unflatten_values \<C> \<V>)
+  case (ev\<^sub>b_jump \<C> p v \<Delta>' p' \<V> \<Delta> s)
+  have "S\<^sub>e (unflatten_closure \<C> v # Lam\<^sub>e (map (unflatten_values \<C>) \<Delta>') (unflatten_code \<C> p') 
+    (alloc_size \<C> p') # unflatten_values \<C> \<V>) ((map (unflatten_values \<C>) \<Delta>, [Jump\<^sub>e]) # 
+    unflatten_stack \<C> s) \<leadsto>\<^sub>e S\<^sub>e (unflatten_values \<C> \<V>) (([unflatten_closure \<C> v] # 
+    map (unflatten_values \<C>) \<Delta>', unflatten_code \<C> p') # unflatten_stack \<C> s)" by (metis ev\<^sub>e_jump)
+  with ev\<^sub>b_jump have "S\<^sub>e (unflatten_closure \<C> v # Lam\<^sub>e (map (unflatten_values \<C>) \<Delta>') 
+    (unflatten_code \<C> p') (alloc_size \<C> p') # unflatten_values \<C> \<V>)
     ((map (unflatten_values \<C>) \<Delta>, unflatten_code \<C> (Suc p)) # unflatten_stack \<C> s) \<leadsto>\<^sub>e
     S\<^sub>e (unflatten_values \<C> \<V>) (([unflatten_closure \<C> v] # map (unflatten_values \<C>) \<Delta>', 
     unflatten_code \<C> p') # unflatten_stack \<C> s)" by simp
-  hence "iter (\<leadsto>\<^sub>e) (S\<^sub>e (unflatten_closure \<C> v # 
-    Lam\<^sub>e (map (unflatten_values \<C>) \<Delta>') (unflatten_code \<C> p') n # unflatten_values \<C> \<V>)
+  hence "iter (\<leadsto>\<^sub>e) (S\<^sub>e (unflatten_closure \<C> v # Lam\<^sub>e (map (unflatten_values \<C>) \<Delta>') 
+    (unflatten_code \<C> p') (alloc_size \<C> p') # unflatten_values \<C> \<V>)
     ((map (unflatten_values \<C>) \<Delta>, unflatten_code \<C> (Suc p)) # unflatten_stack \<C> s))
     (S\<^sub>e (unflatten_values \<C> \<V>) (([unflatten_closure \<C> v] # map (unflatten_values \<C>) \<Delta>', 
     unflatten_code \<C> p') # unflatten_stack \<C> s))" 
       by (metis iter_one)
   thus ?case by simp
-qed
+qed simp_all
 
-text \<open>But it means correctness needs the usual supply of reconstruction lemmas.\<close>
+text \<open>But it means correctness needs the usual supply of reconstruction lemmas. A particular hassle
+is the addition of the \<open>Alloc\<^sub>b\<close> opcodes: we don't have to go as far as we did in stage 4, since we
+can only ever have one \<open>Alloc\<^sub>b\<close> in a row, but it still complicates the lemmas.\<close>
+
+lemma terminated_to_lookup [dest]: "properly_terminated\<^sub>b \<C>\<^sub>b \<Longrightarrow> lookup \<C>\<^sub>b 0 = Some (PushLam\<^sub>b p) \<Longrightarrow> 
+    False"
+  by (induction \<C>\<^sub>b) simp_all
 
 lemma unflatten_to_lookup [dest]: "Lookup\<^sub>e x y # \<C>\<^sub>e = unflatten_code \<C>\<^sub>b (Suc p) \<Longrightarrow> 
-  orderly_code \<C>\<^sub>b 0 \<Longrightarrow> p < length \<C>\<^sub>b \<Longrightarrow> 
-    lookup \<C>\<^sub>b p = Some (Lookup\<^sub>b x y) \<and> \<C>\<^sub>e = unflatten_code \<C>\<^sub>b p"
-  by (simp split: option.splits code\<^sub>b.splits)
+  orderly_code \<C>\<^sub>b 0 \<Longrightarrow> p < length \<C>\<^sub>b \<Longrightarrow> block_structured\<^sub>b \<C>\<^sub>b \<Longrightarrow> 
+    (lookup \<C>\<^sub>b p = Some (Lookup\<^sub>b x y) \<and> \<C>\<^sub>e = unflatten_code \<C>\<^sub>b p) \<or>
+    (\<exists>p' n. p = Suc p' \<and> lookup \<C>\<^sub>b (Suc p') = Some (Alloc\<^sub>b n) \<and> lookup \<C>\<^sub>b p' = Some (Lookup\<^sub>b x y) \<and> 
+      \<C>\<^sub>e = unflatten_code \<C>\<^sub>b p')"
+  by (cases p) (auto split: option.splits code\<^sub>b.splits)
 
 lemma unflatten_to_pushcon [dest]: "PushCon\<^sub>e n # \<C>\<^sub>e = unflatten_code \<C>\<^sub>b (Suc p) \<Longrightarrow> 
-  orderly_code \<C>\<^sub>b 0 \<Longrightarrow> p < length \<C>\<^sub>b \<Longrightarrow> 
-    lookup \<C>\<^sub>b p = Some (PushCon\<^sub>b n) \<and> \<C>\<^sub>e = unflatten_code \<C>\<^sub>b p"
-  by (simp split: option.splits code\<^sub>b.splits)
+  orderly_code \<C>\<^sub>b 0 \<Longrightarrow> p < length \<C>\<^sub>b \<Longrightarrow> block_structured\<^sub>b \<C>\<^sub>b \<Longrightarrow> 
+    (lookup \<C>\<^sub>b p = Some (PushCon\<^sub>b n) \<and> \<C>\<^sub>e = unflatten_code \<C>\<^sub>b p) \<or>
+    (\<exists>p' m. p = Suc p' \<and> lookup \<C>\<^sub>b (Suc p') = Some (Alloc\<^sub>b m) \<and> lookup \<C>\<^sub>b p' = Some (PushCon\<^sub>b n) \<and> 
+      \<C>\<^sub>e = unflatten_code \<C>\<^sub>b p')"
+  by (cases p) (auto split: option.splits code\<^sub>b.splits)
 
 lemma unflatten_to_pushlam [dest]: "PushLam\<^sub>e \<C>\<^sub>e' n # \<C>\<^sub>e = unflatten_code \<C>\<^sub>b (Suc p) \<Longrightarrow> 
-  orderly_code \<C>\<^sub>b 0 \<Longrightarrow> p < length \<C>\<^sub>b \<Longrightarrow>  
-    \<exists>p'. lookup \<C>\<^sub>b p = Some (PushLam\<^sub>b p' n) \<and> \<C>\<^sub>e = unflatten_code \<C>\<^sub>b p \<and> \<C>\<^sub>e' = unflatten_code \<C>\<^sub>b p'"
-  by (simp split: option.splits code\<^sub>b.splits)
+  orderly_code \<C>\<^sub>b 0 \<Longrightarrow> p < length \<C>\<^sub>b \<Longrightarrow> block_structured\<^sub>b \<C>\<^sub>b \<Longrightarrow>
+    \<exists>p'. \<C>\<^sub>e' = unflatten_code \<C>\<^sub>b p' \<and> n = alloc_size \<C>\<^sub>b p' \<and>
+      ((lookup \<C>\<^sub>b p = Some (PushLam\<^sub>b p') \<and> \<C>\<^sub>e = unflatten_code \<C>\<^sub>b p) \<or> 
+      (\<exists>p'' m. p = Suc p'' \<and> lookup \<C>\<^sub>b (Suc p'') = Some (Alloc\<^sub>b m) \<and> 
+        lookup \<C>\<^sub>b p'' = Some (PushLam\<^sub>b p') \<and> \<C>\<^sub>e = unflatten_code \<C>\<^sub>b p''))"
+  by (cases p) (auto split: option.splits code\<^sub>b.splits)
 
 lemma unflatten_to_apply [dest]: "Apply\<^sub>e # \<C>\<^sub>e = unflatten_code \<C>\<^sub>b (Suc p) \<Longrightarrow> orderly_code \<C>\<^sub>b 0 \<Longrightarrow> 
-    p < length \<C>\<^sub>b \<Longrightarrow> lookup \<C>\<^sub>b p = Some Apply\<^sub>b \<and> \<C>\<^sub>e = unflatten_code \<C>\<^sub>b p"
-  by (simp split: option.splits code\<^sub>b.splits)
+    p < length \<C>\<^sub>b \<Longrightarrow> block_structured\<^sub>b \<C>\<^sub>b \<Longrightarrow> 
+      (lookup \<C>\<^sub>b p = Some Apply\<^sub>b \<and> \<C>\<^sub>e = unflatten_code \<C>\<^sub>b p) \<or>
+      (\<exists>p' n. p = Suc p' \<and> lookup \<C>\<^sub>b (Suc p') = Some (Alloc\<^sub>b n) \<and> lookup \<C>\<^sub>b p' = Some Apply\<^sub>b \<and> 
+        \<C>\<^sub>e = unflatten_code \<C>\<^sub>b p')"
+  by (cases p) (auto split: option.splits code\<^sub>b.splits)
 
 lemma unflatten_to_pushenv [dest]: "PushEnv\<^sub>e # \<C>\<^sub>e = unflatten_code \<C>\<^sub>b (Suc p) \<Longrightarrow>
-     orderly_code \<C>\<^sub>b 0 \<Longrightarrow> p < length \<C>\<^sub>b \<Longrightarrow> lookup \<C>\<^sub>b p = Some PushEnv\<^sub>b \<and> \<C>\<^sub>e = unflatten_code \<C>\<^sub>b p"
-  by (simp split: option.splits code\<^sub>b.splits)
+     orderly_code \<C>\<^sub>b 0 \<Longrightarrow> p < length \<C>\<^sub>b \<Longrightarrow> block_structured\<^sub>b \<C>\<^sub>b \<Longrightarrow> 
+      (lookup \<C>\<^sub>b p = Some PushEnv\<^sub>b \<and> \<C>\<^sub>e = unflatten_code \<C>\<^sub>b p) \<or> 
+      (\<exists>p' n. p = Suc p' \<and> lookup \<C>\<^sub>b (Suc p') = Some (Alloc\<^sub>b n) \<and> lookup \<C>\<^sub>b p' = Some PushEnv\<^sub>b \<and> 
+        \<C>\<^sub>e = unflatten_code \<C>\<^sub>b p')"
+  by (cases p) (auto split: option.splits code\<^sub>b.splits)
 
 lemma unflatten_to_return [dest]: "Return\<^sub>e # \<C>\<^sub>e = unflatten_code \<C>\<^sub>b (Suc p) \<Longrightarrow> 
-    orderly_code \<C>\<^sub>b 0 \<Longrightarrow> p < length \<C>\<^sub>b \<Longrightarrow> lookup \<C>\<^sub>b p = Some Return\<^sub>b \<and> \<C>\<^sub>e = []"
-  by (simp split: option.splits code\<^sub>b.splits)
+    orderly_code \<C>\<^sub>b 0 \<Longrightarrow> p < length \<C>\<^sub>b \<Longrightarrow> block_structured\<^sub>b \<C>\<^sub>b \<Longrightarrow> 
+      (lookup \<C>\<^sub>b p = Some Return\<^sub>b \<or> 
+      (\<exists>p' n. p = Suc p' \<and> lookup \<C>\<^sub>b (Suc p') = Some (Alloc\<^sub>b n) \<and> lookup \<C>\<^sub>b p' = Some Return\<^sub>b)) \<and> 
+        \<C>\<^sub>e = []"
+  by (cases p) (auto split: option.splits code\<^sub>b.splits)
 
 lemma unflatten_to_jump [dest]: "Jump\<^sub>e # \<C>\<^sub>e = unflatten_code \<C>\<^sub>b (Suc p) \<Longrightarrow> 
-    orderly_code \<C>\<^sub>b 0 \<Longrightarrow> p < length \<C>\<^sub>b \<Longrightarrow> lookup \<C>\<^sub>b p = Some Jump\<^sub>b \<and> \<C>\<^sub>e = []"
-  by (simp split: option.splits code\<^sub>b.splits)
+    orderly_code \<C>\<^sub>b 0 \<Longrightarrow> p < length \<C>\<^sub>b \<Longrightarrow> block_structured\<^sub>b \<C>\<^sub>b \<Longrightarrow> 
+      (lookup \<C>\<^sub>b p = Some Jump\<^sub>b \<and> \<C>\<^sub>e = []) \<or>
+      (\<exists>p' n. p = Suc p' \<and> lookup \<C>\<^sub>b (Suc p') = Some (Alloc\<^sub>b n) \<and> lookup \<C>\<^sub>b p' = Some Jump\<^sub>b \<and> 
+        \<C>\<^sub>e = [])"
+  by (cases p) (auto split: option.splits code\<^sub>b.splits)
 
 lemma unflatten_stack_to_lookup [dest]: "(\<Delta>\<^sub>e, Lookup\<^sub>e x y # \<C>\<^sub>e) # s\<^sub>e = unflatten_stack \<C>\<^sub>b s\<^sub>b \<Longrightarrow> 
-  orderly_code \<C>\<^sub>b 0 \<Longrightarrow> orderly_stack s\<^sub>b (length \<C>\<^sub>b) \<Longrightarrow> \<exists>\<Delta>\<^sub>b p s\<^sub>b'. 
-    s\<^sub>b = (\<Delta>\<^sub>b, Suc p) # s\<^sub>b' \<and> \<Delta>\<^sub>e = map (unflatten_values \<C>\<^sub>b) \<Delta>\<^sub>b \<and> lookup \<C>\<^sub>b p = Some (Lookup\<^sub>b x y) \<and> 
-      \<C>\<^sub>e = unflatten_code \<C>\<^sub>b p \<and> s\<^sub>e = unflatten_stack \<C>\<^sub>b s\<^sub>b'"
+  orderly_code \<C>\<^sub>b 0 \<Longrightarrow> orderly_stack s\<^sub>b (length \<C>\<^sub>b) \<Longrightarrow> block_structured\<^sub>b \<C>\<^sub>b \<Longrightarrow> \<exists>\<Delta>\<^sub>b p s\<^sub>b'. 
+    s\<^sub>b = (\<Delta>\<^sub>b, Suc p) # s\<^sub>b' \<and> \<Delta>\<^sub>e = map (unflatten_values \<C>\<^sub>b) \<Delta>\<^sub>b \<and> 
+    ((lookup \<C>\<^sub>b p = Some (Lookup\<^sub>b x y) \<and> \<C>\<^sub>e = unflatten_code \<C>\<^sub>b p) \<or>
+    (\<exists>p' n. p = Suc p' \<and> lookup \<C>\<^sub>b (Suc p') = Some (Alloc\<^sub>b n) \<and> lookup \<C>\<^sub>b p' = Some (Lookup\<^sub>b x y) \<and> 
+      \<C>\<^sub>e = unflatten_code \<C>\<^sub>b p')) \<and> s\<^sub>e = unflatten_stack \<C>\<^sub>b s\<^sub>b'"
 proof (induction s\<^sub>b "length \<C>\<^sub>b" rule: orderly_stack.induct)
   case (3 \<Delta>\<^sub>b p s\<^sub>b')
   hence "Lookup\<^sub>e x y # \<C>\<^sub>e = unflatten_code \<C>\<^sub>b (Suc p) \<and> orderly_code \<C>\<^sub>b 0 \<and> p < length \<C>\<^sub>b" by simp
-  hence "lookup \<C>\<^sub>b p = Some (Lookup\<^sub>b x y) \<and> \<C>\<^sub>e = unflatten_code \<C>\<^sub>b p" by blast
+  with 3 have "(lookup \<C>\<^sub>b p = Some (Lookup\<^sub>b x y) \<and> \<C>\<^sub>e = unflatten_code \<C>\<^sub>b p) \<or>
+    (\<exists>p' n. p = Suc p' \<and> lookup \<C>\<^sub>b (Suc p') = Some (Alloc\<^sub>b n) \<and> lookup \<C>\<^sub>b p' = Some (Lookup\<^sub>b x y) \<and> 
+      \<C>\<^sub>e = unflatten_code \<C>\<^sub>b p')" by blast
   with 3 show ?case by simp
 qed simp_all
 
 lemma unflatten_stack_to_pushcon [dest]: "(\<Delta>\<^sub>e, PushCon\<^sub>e n # \<C>\<^sub>e) # s\<^sub>e = unflatten_stack \<C>\<^sub>b s\<^sub>b \<Longrightarrow> 
-  orderly_code \<C>\<^sub>b 0 \<Longrightarrow> orderly_stack s\<^sub>b (length \<C>\<^sub>b) \<Longrightarrow> 
-    \<exists>\<Delta>\<^sub>b p s\<^sub>b'. s\<^sub>b = (\<Delta>\<^sub>b, Suc p) # s\<^sub>b' \<and> \<Delta>\<^sub>e = map (unflatten_values \<C>\<^sub>b) \<Delta>\<^sub>b \<and> 
-      lookup \<C>\<^sub>b p = Some (PushCon\<^sub>b n) \<and> \<C>\<^sub>e = unflatten_code \<C>\<^sub>b p \<and> s\<^sub>e = unflatten_stack \<C>\<^sub>b s\<^sub>b'"
+  orderly_code \<C>\<^sub>b 0 \<Longrightarrow> orderly_stack s\<^sub>b (length \<C>\<^sub>b) \<Longrightarrow> block_structured\<^sub>b \<C>\<^sub>b \<Longrightarrow> \<exists>\<Delta>\<^sub>b p s\<^sub>b'. 
+    s\<^sub>b = (\<Delta>\<^sub>b, Suc p) # s\<^sub>b' \<and> \<Delta>\<^sub>e = map (unflatten_values \<C>\<^sub>b) \<Delta>\<^sub>b \<and> 
+    ((lookup \<C>\<^sub>b p = Some (PushCon\<^sub>b n) \<and> \<C>\<^sub>e = unflatten_code \<C>\<^sub>b p) \<or>
+    (\<exists>p' m. p = Suc p' \<and> lookup \<C>\<^sub>b (Suc p') = Some (Alloc\<^sub>b m) \<and> lookup \<C>\<^sub>b p' = Some (PushCon\<^sub>b n) \<and> 
+      \<C>\<^sub>e = unflatten_code \<C>\<^sub>b p')) \<and> s\<^sub>e = unflatten_stack \<C>\<^sub>b s\<^sub>b'"
 proof (induction s\<^sub>b "length \<C>\<^sub>b" rule: orderly_stack.induct)
   case (3 \<Delta>\<^sub>b p s\<^sub>b')
   hence "PushCon\<^sub>e n # \<C>\<^sub>e = unflatten_code \<C>\<^sub>b (Suc p) \<and> orderly_code \<C>\<^sub>b 0 \<and> p < length \<C>\<^sub>b" by simp
-  hence "lookup \<C>\<^sub>b p = Some (PushCon\<^sub>b n) \<and> \<C>\<^sub>e = unflatten_code \<C>\<^sub>b p" by blast
+  with 3 have "(lookup \<C>\<^sub>b p = Some (PushCon\<^sub>b n) \<and> \<C>\<^sub>e = unflatten_code \<C>\<^sub>b p) \<or>
+    (\<exists>p' m. p = Suc p' \<and> lookup \<C>\<^sub>b (Suc p') = Some (Alloc\<^sub>b m) \<and> lookup \<C>\<^sub>b p' = Some (PushCon\<^sub>b n) \<and> 
+      \<C>\<^sub>e = unflatten_code \<C>\<^sub>b p')" by blast
   with 3 show ?case by simp
 qed simp_all
 
 lemma unflatten_stack_to_pushlam [dest]: "(\<Delta>\<^sub>e, PushLam\<^sub>e \<C>\<^sub>e' n # \<C>\<^sub>e) # s\<^sub>e = unflatten_stack \<C>\<^sub>b s\<^sub>b \<Longrightarrow> 
-  orderly_code \<C>\<^sub>b 0 \<Longrightarrow> orderly_stack s\<^sub>b (length \<C>\<^sub>b) \<Longrightarrow> \<exists>\<Delta>\<^sub>b p s\<^sub>b' p'. 
-  s\<^sub>b = (\<Delta>\<^sub>b, Suc p) # s\<^sub>b' \<and> \<Delta>\<^sub>e = map (unflatten_values \<C>\<^sub>b) \<Delta>\<^sub>b \<and> lookup \<C>\<^sub>b p = Some (PushLam\<^sub>b p' n) \<and> 
-  \<C>\<^sub>e = unflatten_code \<C>\<^sub>b p \<and> \<C>\<^sub>e' = unflatten_code \<C>\<^sub>b p' \<and> s\<^sub>e = unflatten_stack \<C>\<^sub>b s\<^sub>b'"
+  orderly_code \<C>\<^sub>b 0 \<Longrightarrow> orderly_stack s\<^sub>b (length \<C>\<^sub>b) \<Longrightarrow> block_structured\<^sub>b \<C>\<^sub>b \<Longrightarrow> \<exists>\<Delta>\<^sub>b p s\<^sub>b' p'. 
+  s\<^sub>b = (\<Delta>\<^sub>b, Suc p) # s\<^sub>b' \<and> \<Delta>\<^sub>e = map (unflatten_values \<C>\<^sub>b) \<Delta>\<^sub>b \<and> \<C>\<^sub>e' = unflatten_code \<C>\<^sub>b p' \<and> 
+    n = alloc_size \<C>\<^sub>b p' \<and> ((lookup \<C>\<^sub>b p = Some (PushLam\<^sub>b p') \<and> \<C>\<^sub>e = unflatten_code \<C>\<^sub>b p) \<or> 
+    (\<exists>p'' m. p = Suc p'' \<and> lookup \<C>\<^sub>b (Suc p'') = Some (Alloc\<^sub>b m) \<and> 
+      lookup \<C>\<^sub>b p'' = Some (PushLam\<^sub>b p') \<and> \<C>\<^sub>e = unflatten_code \<C>\<^sub>b p'')) \<and> 
+  s\<^sub>e = unflatten_stack \<C>\<^sub>b s\<^sub>b'"
 proof (induction s\<^sub>b "length \<C>\<^sub>b" rule: orderly_stack.induct)
   case (3 \<Delta>\<^sub>b p s\<^sub>b')
   hence "PushLam\<^sub>e \<C>\<^sub>e' n # \<C>\<^sub>e = unflatten_code \<C>\<^sub>b (Suc p) \<and> orderly_code \<C>\<^sub>b 0 \<and> p < length \<C>\<^sub>b" 
     by simp
-  then obtain p' where "lookup \<C>\<^sub>b p = Some (PushLam\<^sub>b p' n) \<and> \<C>\<^sub>e = unflatten_code \<C>\<^sub>b p \<and> 
-    \<C>\<^sub>e' = unflatten_code \<C>\<^sub>b p'" by blast
-  with 3 show ?case by simp
+  with 3 obtain p' where P: "\<C>\<^sub>e' = unflatten_code \<C>\<^sub>b p' \<and> n = alloc_size \<C>\<^sub>b p' \<and>
+    ((lookup \<C>\<^sub>b p = Some (PushLam\<^sub>b p') \<and> \<C>\<^sub>e = unflatten_code \<C>\<^sub>b p) \<or> 
+    (\<exists>p'' m. p = Suc p'' \<and> lookup \<C>\<^sub>b (Suc p'') = Some (Alloc\<^sub>b m) \<and> 
+      lookup \<C>\<^sub>b p'' = Some (PushLam\<^sub>b p') \<and> \<C>\<^sub>e = unflatten_code \<C>\<^sub>b p''))" by blast
+  from 3 have "\<Delta>\<^sub>e = map (unflatten_values \<C>\<^sub>b) \<Delta>\<^sub>b \<and> s\<^sub>e = unflatten_stack \<C>\<^sub>b s\<^sub>b'" by simp
+  with 3 P show ?case by blast
 qed simp_all
 
 lemma unflatten_stack_to_apply [dest]: "(\<Delta>\<^sub>e, Apply\<^sub>e # \<C>\<^sub>e) # s\<^sub>e = unflatten_stack \<C>\<^sub>b s\<^sub>b \<Longrightarrow> 
-  orderly_code \<C>\<^sub>b 0 \<Longrightarrow> orderly_stack s\<^sub>b (length \<C>\<^sub>b) \<Longrightarrow> \<exists>\<Delta>\<^sub>b p s\<^sub>b'. s\<^sub>b = (\<Delta>\<^sub>b, Suc p) # s\<^sub>b' \<and> 
-    \<Delta>\<^sub>e = map (unflatten_values \<C>\<^sub>b) \<Delta>\<^sub>b \<and> lookup \<C>\<^sub>b p = Some Apply\<^sub>b \<and> \<C>\<^sub>e = unflatten_code \<C>\<^sub>b p \<and> 
-      s\<^sub>e = unflatten_stack \<C>\<^sub>b s\<^sub>b'"
+  orderly_code \<C>\<^sub>b 0 \<Longrightarrow> orderly_stack s\<^sub>b (length \<C>\<^sub>b) \<Longrightarrow> block_structured\<^sub>b \<C>\<^sub>b \<Longrightarrow> \<exists>\<Delta>\<^sub>b p s\<^sub>b'. 
+    s\<^sub>b = (\<Delta>\<^sub>b, Suc p) # s\<^sub>b' \<and> \<Delta>\<^sub>e = map (unflatten_values \<C>\<^sub>b) \<Delta>\<^sub>b \<and> 
+      ((lookup \<C>\<^sub>b p = Some Apply\<^sub>b \<and> \<C>\<^sub>e = unflatten_code \<C>\<^sub>b p) \<or>
+      (\<exists>p' n. p = Suc p' \<and> lookup \<C>\<^sub>b (Suc p') = Some (Alloc\<^sub>b n) \<and> lookup \<C>\<^sub>b p' = Some Apply\<^sub>b \<and> 
+        \<C>\<^sub>e = unflatten_code \<C>\<^sub>b p')) \<and> s\<^sub>e = unflatten_stack \<C>\<^sub>b s\<^sub>b'"
 proof (induction s\<^sub>b "length \<C>\<^sub>b" rule: orderly_stack.induct)
   case (3 \<Delta>\<^sub>b p s\<^sub>b')
   hence "Apply\<^sub>e # \<C>\<^sub>e = unflatten_code \<C>\<^sub>b (Suc p) \<and> orderly_code \<C>\<^sub>b 0 \<and> p < length \<C>\<^sub>b" by simp
-  hence "lookup \<C>\<^sub>b p = Some Apply\<^sub>b \<and> \<C>\<^sub>e = unflatten_code \<C>\<^sub>b p" by blast
+  with 3 have "(lookup \<C>\<^sub>b p = Some Apply\<^sub>b \<and> \<C>\<^sub>e = unflatten_code \<C>\<^sub>b p) \<or>
+      (\<exists>p' n. p = Suc p' \<and> lookup \<C>\<^sub>b (Suc p') = Some (Alloc\<^sub>b n) \<and> lookup \<C>\<^sub>b p' = Some Apply\<^sub>b \<and> 
+        \<C>\<^sub>e = unflatten_code \<C>\<^sub>b p')" by blast
   with 3 show ?case by simp
 qed simp_all
 
 lemma unflatten_stack_to_pushenv [dest]: "(\<Delta>\<^sub>e, PushEnv\<^sub>e # \<C>\<^sub>e) # s\<^sub>e = unflatten_stack \<C>\<^sub>b s\<^sub>b \<Longrightarrow> 
-  orderly_code \<C>\<^sub>b 0 \<Longrightarrow> orderly_stack s\<^sub>b (length \<C>\<^sub>b) \<Longrightarrow> \<exists>\<Delta>\<^sub>b p s\<^sub>b'. s\<^sub>b = (\<Delta>\<^sub>b, Suc p) # s\<^sub>b' \<and> 
-    \<Delta>\<^sub>e = map (unflatten_values \<C>\<^sub>b) \<Delta>\<^sub>b \<and> lookup \<C>\<^sub>b p = Some PushEnv\<^sub>b \<and> \<C>\<^sub>e = unflatten_code \<C>\<^sub>b p \<and> 
-      s\<^sub>e = unflatten_stack \<C>\<^sub>b s\<^sub>b'"
+  orderly_code \<C>\<^sub>b 0 \<Longrightarrow> orderly_stack s\<^sub>b (length \<C>\<^sub>b) \<Longrightarrow> block_structured\<^sub>b \<C>\<^sub>b \<Longrightarrow>  \<exists>\<Delta>\<^sub>b p s\<^sub>b'. 
+    s\<^sub>b = (\<Delta>\<^sub>b, Suc p) # s\<^sub>b' \<and> \<Delta>\<^sub>e = map (unflatten_values \<C>\<^sub>b) \<Delta>\<^sub>b \<and> 
+      ((lookup \<C>\<^sub>b p = Some PushEnv\<^sub>b \<and> \<C>\<^sub>e = unflatten_code \<C>\<^sub>b p) \<or>
+      (\<exists>p' n. p = Suc p' \<and> lookup \<C>\<^sub>b (Suc p') = Some (Alloc\<^sub>b n) \<and> lookup \<C>\<^sub>b p' = Some PushEnv\<^sub>b \<and> 
+        \<C>\<^sub>e = unflatten_code \<C>\<^sub>b p')) \<and> s\<^sub>e = unflatten_stack \<C>\<^sub>b s\<^sub>b'"
 proof (induction s\<^sub>b "length \<C>\<^sub>b" rule: orderly_stack.induct)
   case (3 \<Delta>\<^sub>b p s\<^sub>b')
   hence "PushEnv\<^sub>e # \<C>\<^sub>e = unflatten_code \<C>\<^sub>b (Suc p) \<and> orderly_code \<C>\<^sub>b 0 \<and> p < length \<C>\<^sub>b" by simp
-  hence "lookup \<C>\<^sub>b p = Some PushEnv\<^sub>b \<and> \<C>\<^sub>e = unflatten_code \<C>\<^sub>b p" by blast
+  with 3 have "(lookup \<C>\<^sub>b p = Some PushEnv\<^sub>b \<and> \<C>\<^sub>e = unflatten_code \<C>\<^sub>b p) \<or>
+      (\<exists>p' n. p = Suc p' \<and> lookup \<C>\<^sub>b (Suc p') = Some (Alloc\<^sub>b n) \<and> lookup \<C>\<^sub>b p' = Some PushEnv\<^sub>b \<and> 
+        \<C>\<^sub>e = unflatten_code \<C>\<^sub>b p')" by blast
   with 3 show ?case by simp
 qed simp_all
 
 lemma unflatten_stack_to_return [dest]: "(\<Delta>\<^sub>e, Return\<^sub>e # \<C>\<^sub>e) # s\<^sub>e = unflatten_stack \<C>\<^sub>b s\<^sub>b \<Longrightarrow> 
-  orderly_code \<C>\<^sub>b 0 \<Longrightarrow> orderly_stack s\<^sub>b (length \<C>\<^sub>b) \<Longrightarrow> \<exists>\<Delta>\<^sub>b p s\<^sub>b'. s\<^sub>b = (\<Delta>\<^sub>b, Suc p) # s\<^sub>b' \<and> 
-    \<Delta>\<^sub>e = map (unflatten_values \<C>\<^sub>b) \<Delta>\<^sub>b \<and> lookup \<C>\<^sub>b p = Some Return\<^sub>b \<and> s\<^sub>e = unflatten_stack \<C>\<^sub>b s\<^sub>b' \<and> 
-      \<C>\<^sub>e = []"
+  orderly_code \<C>\<^sub>b 0 \<Longrightarrow> orderly_stack s\<^sub>b (length \<C>\<^sub>b) \<Longrightarrow> block_structured\<^sub>b \<C>\<^sub>b \<Longrightarrow> \<exists>\<Delta>\<^sub>b p s\<^sub>b'. 
+    s\<^sub>b = (\<Delta>\<^sub>b, Suc p) # s\<^sub>b' \<and> \<Delta>\<^sub>e = map (unflatten_values \<C>\<^sub>b) \<Delta>\<^sub>b \<and> 
+      (lookup \<C>\<^sub>b p = Some Return\<^sub>b \<or> 
+      (\<exists>p' n. p = Suc p' \<and> lookup \<C>\<^sub>b (Suc p') = Some (Alloc\<^sub>b n) \<and> lookup \<C>\<^sub>b p' = Some Return\<^sub>b)) \<and> 
+        \<C>\<^sub>e = [] \<and> s\<^sub>e = unflatten_stack \<C>\<^sub>b s\<^sub>b'"
 proof (induction s\<^sub>b "length \<C>\<^sub>b" rule: orderly_stack.induct)
   case (3 \<Delta>\<^sub>b p s\<^sub>b')
   hence "Return\<^sub>e # \<C>\<^sub>e = unflatten_code \<C>\<^sub>b (Suc p) \<and> orderly_code \<C>\<^sub>b 0 \<and> p < length \<C>\<^sub>b" by simp
-  hence "lookup \<C>\<^sub>b p = Some Return\<^sub>b \<and> \<C>\<^sub>e = []" by blast
+  with 3 have "(lookup \<C>\<^sub>b p = Some Return\<^sub>b \<or> 
+      (\<exists>p' n. p = Suc p' \<and> lookup \<C>\<^sub>b (Suc p') = Some (Alloc\<^sub>b n) \<and> lookup \<C>\<^sub>b p' = Some Return\<^sub>b)) \<and> 
+        \<C>\<^sub>e = []" by blast
   with 3 show ?case by simp
 qed simp_all
 
 lemma unflatten_stack_to_jump [dest]: "(\<Delta>\<^sub>e, Jump\<^sub>e # \<C>\<^sub>e) # s\<^sub>e = unflatten_stack \<C>\<^sub>b s\<^sub>b \<Longrightarrow> 
-  orderly_code \<C>\<^sub>b 0 \<Longrightarrow> orderly_stack s\<^sub>b (length \<C>\<^sub>b) \<Longrightarrow> \<exists>\<Delta>\<^sub>b p s\<^sub>b'. s\<^sub>b = (\<Delta>\<^sub>b, Suc p) # s\<^sub>b' \<and> 
-    \<Delta>\<^sub>e = map (unflatten_values \<C>\<^sub>b) \<Delta>\<^sub>b \<and> lookup \<C>\<^sub>b p = Some Jump\<^sub>b \<and> s\<^sub>e = unflatten_stack \<C>\<^sub>b s\<^sub>b'"
+  orderly_code \<C>\<^sub>b 0 \<Longrightarrow> orderly_stack s\<^sub>b (length \<C>\<^sub>b) \<Longrightarrow> block_structured\<^sub>b \<C>\<^sub>b \<Longrightarrow> \<exists>\<Delta>\<^sub>b p s\<^sub>b'. 
+    s\<^sub>b = (\<Delta>\<^sub>b, Suc p) # s\<^sub>b' \<and> \<Delta>\<^sub>e = map (unflatten_values \<C>\<^sub>b) \<Delta>\<^sub>b \<and> (lookup \<C>\<^sub>b p = Some Jump\<^sub>b \<or> 
+      (\<exists>p' n. p = Suc p' \<and> lookup \<C>\<^sub>b (Suc p') = Some (Alloc\<^sub>b n) \<and> lookup \<C>\<^sub>b p' = Some Jump\<^sub>b)) \<and> 
+        \<C>\<^sub>e = [] \<and> s\<^sub>e = unflatten_stack \<C>\<^sub>b s\<^sub>b'"
 proof (induction s\<^sub>b "length \<C>\<^sub>b" rule: orderly_stack.induct)
   case (3 \<Delta>\<^sub>b p s\<^sub>b')
   hence "Jump\<^sub>e # \<C>\<^sub>e = unflatten_code \<C>\<^sub>b (Suc p) \<and> orderly_code \<C>\<^sub>b 0 \<and> p < length \<C>\<^sub>b" by simp
-  hence "lookup \<C>\<^sub>b p = Some Jump\<^sub>b \<and> \<C>\<^sub>e = []" by blast
+  with 3 have "(lookup \<C>\<^sub>b p = Some Jump\<^sub>b \<or> 
+      (\<exists>p' n. p = Suc p' \<and> lookup \<C>\<^sub>b (Suc p') = Some (Alloc\<^sub>b n) \<and> lookup \<C>\<^sub>b p' = Some Jump\<^sub>b)) \<and> 
+        \<C>\<^sub>e = []" by blast
   with 3 show ?case by simp
 qed simp_all
 
 lemma unflatten_to_lam [dest]: "Lam\<^sub>e \<Delta>\<^sub>e \<C>\<^sub>e n = unflatten_closure \<C>\<^sub>b v\<^sub>b \<Longrightarrow> 
-    \<exists>\<Delta>\<^sub>b p. v\<^sub>b = Lam\<^sub>b \<Delta>\<^sub>b p n \<and> \<Delta>\<^sub>e = map (unflatten_values \<C>\<^sub>b) \<Delta>\<^sub>b \<and> \<C>\<^sub>e = unflatten_code \<C>\<^sub>b p"
+    \<exists>\<Delta>\<^sub>b p. v\<^sub>b = Lam\<^sub>b \<Delta>\<^sub>b p \<and> \<Delta>\<^sub>e = map (unflatten_values \<C>\<^sub>b) \<Delta>\<^sub>b \<and> \<C>\<^sub>e = unflatten_code \<C>\<^sub>b p \<and> 
+      n = alloc_size \<C>\<^sub>b p"
   by (induction v\<^sub>b) simp_all
 
 lemma unflatten_state [dest]: "S\<^sub>e \<V>\<^sub>e s\<^sub>e = unflatten_state \<C> \<Sigma>\<^sub>b \<Longrightarrow> \<exists>\<V>\<^sub>b s\<^sub>b. 
@@ -445,99 +518,218 @@ proof (induction "unflatten_state \<C>\<^sub>b \<Sigma>\<^sub>b" \<Sigma>\<^sub>
   case (ev\<^sub>e_lookup \<Delta>\<^sub>e x vs y v \<V>\<^sub>e \<C>\<^sub>e s\<^sub>e)
   then obtain \<V>\<^sub>b s\<^sub>b where B: "\<Sigma>\<^sub>b = S\<^sub>b \<V>\<^sub>b s\<^sub>b \<and> \<V>\<^sub>e = unflatten_values \<C>\<^sub>b \<V>\<^sub>b \<and> 
     (\<Delta>\<^sub>e, Lookup\<^sub>e x y # \<C>\<^sub>e) # s\<^sub>e = unflatten_stack \<C>\<^sub>b s\<^sub>b" by fastforce
-  with ev\<^sub>e_lookup have "orderly_code \<C>\<^sub>b 0 \<and> orderly_stack s\<^sub>b (length \<C>\<^sub>b)" by simp
+  with ev\<^sub>e_lookup have "orderly_code \<C>\<^sub>b 0 \<and> orderly_stack s\<^sub>b (length \<C>\<^sub>b) \<and> block_structured\<^sub>b \<C>\<^sub>b" 
+    by simp
   with B obtain \<Delta>\<^sub>b p s\<^sub>b' where S: "s\<^sub>b = (\<Delta>\<^sub>b, Suc p) # s\<^sub>b' \<and> 
-    \<Delta>\<^sub>e = map (unflatten_values \<C>\<^sub>b) \<Delta>\<^sub>b \<and> lookup \<C>\<^sub>b p = Some (Lookup\<^sub>b x y) \<and> 
-    \<C>\<^sub>e = unflatten_code \<C>\<^sub>b p \<and> s\<^sub>e = unflatten_stack \<C>\<^sub>b s\<^sub>b'" by (metis unflatten_stack_to_lookup)
+    \<Delta>\<^sub>e = map (unflatten_values \<C>\<^sub>b) \<Delta>\<^sub>b \<and> ((lookup \<C>\<^sub>b p = Some (Lookup\<^sub>b x y) \<and> 
+    \<C>\<^sub>e = unflatten_code \<C>\<^sub>b p) \<or> (\<exists>p' n. p = Suc p' \<and> lookup \<C>\<^sub>b p = Some (Alloc\<^sub>b n) \<and> 
+    lookup \<C>\<^sub>b p' = Some (Lookup\<^sub>b x y) \<and> \<C>\<^sub>e = unflatten_code \<C>\<^sub>b p')) \<and> s\<^sub>e = unflatten_stack \<C>\<^sub>b s\<^sub>b'" 
+      by (metis unflatten_stack_to_lookup)
   with ev\<^sub>e_lookup obtain vs' where VS: "lookup \<Delta>\<^sub>b x = Some vs' \<and> 
     map (unflatten_closure \<C>\<^sub>b) vs' = vs" by fastforce
   with ev\<^sub>e_lookup obtain v' where V: "lookup vs' y = Some v' \<and> unflatten_closure \<C>\<^sub>b v' = v" 
     by fastforce
-  with S VS have "\<C>\<^sub>b \<tturnstile> S\<^sub>b \<V>\<^sub>b ((\<Delta>\<^sub>b, Suc p) # s\<^sub>b') \<leadsto>\<^sub>b S\<^sub>b (v' # \<V>\<^sub>b) ((\<Delta>\<^sub>b, p) # s\<^sub>b')" by simp
-  hence "iter (\<tturnstile> \<C>\<^sub>b \<leadsto>\<^sub>b) (S\<^sub>b \<V>\<^sub>b ((\<Delta>\<^sub>b, Suc p) # s\<^sub>b')) (S\<^sub>b (v' # \<V>\<^sub>b) ((\<Delta>\<^sub>b, p) # s\<^sub>b'))" by simp
-  with B S VS V show ?case by fastforce
+  show ?case
+  proof (cases "lookup \<C>\<^sub>b p = Some (Lookup\<^sub>b x y) \<and> \<C>\<^sub>e = unflatten_code \<C>\<^sub>b p")
+    case True
+    with S VS V have "\<C>\<^sub>b \<tturnstile> S\<^sub>b \<V>\<^sub>b ((\<Delta>\<^sub>b, Suc p) # s\<^sub>b') \<leadsto>\<^sub>b S\<^sub>b (v' # \<V>\<^sub>b) ((\<Delta>\<^sub>b, p) # s\<^sub>b')" by simp
+    hence "iter (\<tturnstile> \<C>\<^sub>b \<leadsto>\<^sub>b) (S\<^sub>b \<V>\<^sub>b ((\<Delta>\<^sub>b, Suc p) # s\<^sub>b')) (S\<^sub>b (v' # \<V>\<^sub>b) ((\<Delta>\<^sub>b, p) # s\<^sub>b'))" by simp
+    with B S VS V True show ?thesis by fastforce
+  next
+    case False
+    with S obtain p' n where P: "p = Suc p' \<and> lookup \<C>\<^sub>b (Suc p') = Some (Alloc\<^sub>b n) \<and> 
+      lookup \<C>\<^sub>b p' = Some (Lookup\<^sub>b x y) \<and> \<C>\<^sub>e = unflatten_code \<C>\<^sub>b p'" by blast
+    with VS V have "\<C>\<^sub>b \<tturnstile> S\<^sub>b \<V>\<^sub>b ((\<Delta>\<^sub>b, Suc p') # s\<^sub>b') \<leadsto>\<^sub>b S\<^sub>b (v' # \<V>\<^sub>b) ((\<Delta>\<^sub>b, p') # s\<^sub>b')" by simp
+    moreover from P have "\<C>\<^sub>b \<tturnstile> S\<^sub>b \<V>\<^sub>b ((\<Delta>\<^sub>b, Suc (Suc p')) # s\<^sub>b') \<leadsto>\<^sub>b S\<^sub>b \<V>\<^sub>b ((\<Delta>\<^sub>b, Suc p') # s\<^sub>b')" 
+      by simp
+    ultimately have "iter (\<tturnstile> \<C>\<^sub>b \<leadsto>\<^sub>b) (S\<^sub>b \<V>\<^sub>b ((\<Delta>\<^sub>b, Suc (Suc p')) # s\<^sub>b')) 
+      (S\<^sub>b (v' # \<V>\<^sub>b) ((\<Delta>\<^sub>b, p') # s\<^sub>b'))" by (metis iter_step iter_refl)
+    with B S VS V False P show ?thesis by fastforce
+  qed
 next
   case (ev\<^sub>e_pushcon \<V>\<^sub>e \<Delta>\<^sub>e n \<C>\<^sub>e s\<^sub>e)
   then obtain \<V>\<^sub>b s\<^sub>b where B: "\<Sigma>\<^sub>b = S\<^sub>b \<V>\<^sub>b s\<^sub>b \<and> \<V>\<^sub>e = unflatten_values \<C>\<^sub>b \<V>\<^sub>b \<and> 
     (\<Delta>\<^sub>e, PushCon\<^sub>e n # \<C>\<^sub>e) # s\<^sub>e = unflatten_stack \<C>\<^sub>b s\<^sub>b" by fastforce
-  with ev\<^sub>e_pushcon have "orderly_code \<C>\<^sub>b 0 \<and> orderly_stack s\<^sub>b (length \<C>\<^sub>b)" by simp
-  with B obtain \<Delta>\<^sub>b p s\<^sub>b' where S: "s\<^sub>b = (\<Delta>\<^sub>b, Suc p) # s\<^sub>b' \<and> 
-    \<Delta>\<^sub>e = map (unflatten_values \<C>\<^sub>b) \<Delta>\<^sub>b \<and> lookup \<C>\<^sub>b p = Some (PushCon\<^sub>b n) \<and> \<C>\<^sub>e = unflatten_code \<C>\<^sub>b p \<and> 
-      s\<^sub>e = unflatten_stack \<C>\<^sub>b s\<^sub>b'" by (metis unflatten_stack_to_pushcon)
-  with S have "\<C>\<^sub>b \<tturnstile> S\<^sub>b \<V>\<^sub>b ((\<Delta>\<^sub>b, Suc p) # s\<^sub>b') \<leadsto>\<^sub>b S\<^sub>b (Const\<^sub>b n # \<V>\<^sub>b) ((\<Delta>\<^sub>b, p) # s\<^sub>b')" by simp
-  hence "iter (\<tturnstile> \<C>\<^sub>b \<leadsto>\<^sub>b) (S\<^sub>b \<V>\<^sub>b ((\<Delta>\<^sub>b, Suc p) # s\<^sub>b')) (S\<^sub>b (Const\<^sub>b n # \<V>\<^sub>b) ((\<Delta>\<^sub>b, p) # s\<^sub>b'))" by simp
-  with B S show ?case by fastforce
+  with ev\<^sub>e_pushcon have "orderly_code \<C>\<^sub>b 0 \<and> orderly_stack s\<^sub>b (length \<C>\<^sub>b) \<and> block_structured\<^sub>b \<C>\<^sub>b" 
+    by simp
+  with B obtain \<Delta>\<^sub>b p s\<^sub>b' where S: "s\<^sub>b = (\<Delta>\<^sub>b, Suc p) # s\<^sub>b' \<and> \<Delta>\<^sub>e = map (unflatten_values \<C>\<^sub>b) \<Delta>\<^sub>b \<and> 
+    ((lookup \<C>\<^sub>b p = Some (PushCon\<^sub>b n) \<and> \<C>\<^sub>e = unflatten_code \<C>\<^sub>b p) \<or>
+    (\<exists>p' m. p = Suc p' \<and> lookup \<C>\<^sub>b (Suc p') = Some (Alloc\<^sub>b m) \<and> lookup \<C>\<^sub>b p' = Some (PushCon\<^sub>b n) \<and> 
+      \<C>\<^sub>e = unflatten_code \<C>\<^sub>b p')) \<and> s\<^sub>e = unflatten_stack \<C>\<^sub>b s\<^sub>b'" by (metis unflatten_stack_to_pushcon)
+  show ?case
+  proof (cases "lookup \<C>\<^sub>b p = Some (PushCon\<^sub>b n) \<and> \<C>\<^sub>e = unflatten_code \<C>\<^sub>b p")
+    case True
+    with S have "\<C>\<^sub>b \<tturnstile> S\<^sub>b \<V>\<^sub>b ((\<Delta>\<^sub>b, Suc p) # s\<^sub>b') \<leadsto>\<^sub>b S\<^sub>b (Const\<^sub>b n # \<V>\<^sub>b) ((\<Delta>\<^sub>b, p) # s\<^sub>b')" by simp
+    hence "iter (\<tturnstile> \<C>\<^sub>b \<leadsto>\<^sub>b) (S\<^sub>b \<V>\<^sub>b ((\<Delta>\<^sub>b, Suc p) # s\<^sub>b')) (S\<^sub>b (Const\<^sub>b n # \<V>\<^sub>b) ((\<Delta>\<^sub>b, p) # s\<^sub>b'))" by simp
+    with B S True show ?thesis by fastforce
+  next
+    case False
+    with S obtain p' m where P: "p = Suc p' \<and> lookup \<C>\<^sub>b (Suc p') = Some (Alloc\<^sub>b m) \<and> 
+      lookup \<C>\<^sub>b p' = Some (PushCon\<^sub>b n) \<and> \<C>\<^sub>e = unflatten_code \<C>\<^sub>b p'" by blast
+    with S have "\<C>\<^sub>b \<tturnstile> S\<^sub>b \<V>\<^sub>b ((\<Delta>\<^sub>b, Suc (Suc p')) # s\<^sub>b') \<leadsto>\<^sub>b S\<^sub>b \<V>\<^sub>b ((\<Delta>\<^sub>b, Suc p') # s\<^sub>b')" by simp
+    moreover from S P have "\<C>\<^sub>b \<tturnstile> S\<^sub>b \<V>\<^sub>b ((\<Delta>\<^sub>b, Suc p') # s\<^sub>b') \<leadsto>\<^sub>b S\<^sub>b (Const\<^sub>b n # \<V>\<^sub>b) ((\<Delta>\<^sub>b, p') # s\<^sub>b')" 
+      by simp
+    ultimately have "iter (\<tturnstile> \<C>\<^sub>b \<leadsto>\<^sub>b) (S\<^sub>b \<V>\<^sub>b ((\<Delta>\<^sub>b, Suc (Suc p')) # s\<^sub>b')) 
+      (S\<^sub>b (Const\<^sub>b n # \<V>\<^sub>b) ((\<Delta>\<^sub>b, p') # s\<^sub>b'))" by (metis iter_step iter_refl)
+    with B S False P show ?thesis by fastforce
+  qed
 next
   case (ev\<^sub>e_pushlam \<V>\<^sub>e \<Delta>\<^sub>e \<C>\<^sub>e' n \<C>\<^sub>e s\<^sub>e)
   then obtain \<V>\<^sub>b s\<^sub>b where B: "\<Sigma>\<^sub>b = S\<^sub>b \<V>\<^sub>b s\<^sub>b \<and> \<V>\<^sub>e = unflatten_values \<C>\<^sub>b \<V>\<^sub>b \<and> 
     (\<Delta>\<^sub>e, PushLam\<^sub>e \<C>\<^sub>e' n # \<C>\<^sub>e) # s\<^sub>e = unflatten_stack \<C>\<^sub>b s\<^sub>b" by fastforce
-  with ev\<^sub>e_pushlam have "orderly_code \<C>\<^sub>b 0 \<and> orderly_stack s\<^sub>b (length \<C>\<^sub>b)" by simp
-  with B obtain \<Delta>\<^sub>b p s\<^sub>b' p' where S: "s\<^sub>b = (\<Delta>\<^sub>b, Suc p) # s\<^sub>b' \<and> 
-    \<Delta>\<^sub>e = map (unflatten_values \<C>\<^sub>b) \<Delta>\<^sub>b \<and> lookup \<C>\<^sub>b p = Some (PushLam\<^sub>b p' n) \<and> 
-      \<C>\<^sub>e = unflatten_code \<C>\<^sub>b p \<and> s\<^sub>e = unflatten_stack \<C>\<^sub>b s\<^sub>b' \<and> \<C>\<^sub>e' = unflatten_code \<C>\<^sub>b p'" 
-    by (metis unflatten_stack_to_pushlam)
-  with S have "\<C>\<^sub>b \<tturnstile> S\<^sub>b \<V>\<^sub>b ((\<Delta>\<^sub>b, Suc p) # s\<^sub>b') \<leadsto>\<^sub>b S\<^sub>b (Lam\<^sub>b \<Delta>\<^sub>b p' n # \<V>\<^sub>b) ((\<Delta>\<^sub>b, p) # s\<^sub>b')" by simp
-  hence "iter (\<tturnstile> \<C>\<^sub>b \<leadsto>\<^sub>b) (S\<^sub>b \<V>\<^sub>b ((\<Delta>\<^sub>b, Suc p) # s\<^sub>b')) (S\<^sub>b (Lam\<^sub>b \<Delta>\<^sub>b p' n # \<V>\<^sub>b) ((\<Delta>\<^sub>b, p) # s\<^sub>b'))" 
+  with ev\<^sub>e_pushlam have "orderly_code \<C>\<^sub>b 0 \<and> orderly_stack s\<^sub>b (length \<C>\<^sub>b) \<and> block_structured\<^sub>b \<C>\<^sub>b" 
     by simp
-  with B S show ?case by fastforce
+  with B obtain \<Delta>\<^sub>b p s\<^sub>b' p' where S: "s\<^sub>b = (\<Delta>\<^sub>b, Suc p) # s\<^sub>b' \<and> \<Delta>\<^sub>e = map (unflatten_values \<C>\<^sub>b) \<Delta>\<^sub>b \<and> 
+    \<C>\<^sub>e' = unflatten_code \<C>\<^sub>b p' \<and> n = alloc_size \<C>\<^sub>b p' \<and> ((lookup \<C>\<^sub>b p = Some (PushLam\<^sub>b p') \<and> 
+    \<C>\<^sub>e = unflatten_code \<C>\<^sub>b p) \<or> (\<exists>p'' m. p = Suc p'' \<and> lookup \<C>\<^sub>b (Suc p'') = Some (Alloc\<^sub>b m) \<and> 
+      lookup \<C>\<^sub>b p'' = Some (PushLam\<^sub>b p') \<and> \<C>\<^sub>e = unflatten_code \<C>\<^sub>b p'')) \<and> s\<^sub>e = unflatten_stack \<C>\<^sub>b s\<^sub>b'"
+    using unflatten_stack_to_pushlam by metis
+  show ?case
+  proof (cases "lookup \<C>\<^sub>b p = Some (PushLam\<^sub>b p') \<and> \<C>\<^sub>e = unflatten_code \<C>\<^sub>b p")
+    case True
+    with S have "\<C>\<^sub>b \<tturnstile> S\<^sub>b \<V>\<^sub>b ((\<Delta>\<^sub>b, Suc p) # s\<^sub>b') \<leadsto>\<^sub>b S\<^sub>b (Lam\<^sub>b \<Delta>\<^sub>b p' # \<V>\<^sub>b) ((\<Delta>\<^sub>b, p) # s\<^sub>b')" by simp
+    hence "iter (\<tturnstile> \<C>\<^sub>b \<leadsto>\<^sub>b) (S\<^sub>b \<V>\<^sub>b ((\<Delta>\<^sub>b, Suc p) # s\<^sub>b')) (S\<^sub>b (Lam\<^sub>b \<Delta>\<^sub>b p' # \<V>\<^sub>b) ((\<Delta>\<^sub>b, p) # s\<^sub>b'))" 
+      by simp
+    with B S True show ?thesis by fastforce
+  next
+    case False
+    with S obtain p'' m where P: "p = Suc p'' \<and> lookup \<C>\<^sub>b (Suc p'') = Some (Alloc\<^sub>b m) \<and> 
+      lookup \<C>\<^sub>b p'' = Some (PushLam\<^sub>b p') \<and> \<C>\<^sub>e = unflatten_code \<C>\<^sub>b p''" by blast
+    with S have "\<C>\<^sub>b \<tturnstile> S\<^sub>b \<V>\<^sub>b ((\<Delta>\<^sub>b, Suc (Suc p'')) # s\<^sub>b') \<leadsto>\<^sub>b S\<^sub>b \<V>\<^sub>b ((\<Delta>\<^sub>b, Suc p'') # s\<^sub>b')" by simp
+    moreover from S P have "\<C>\<^sub>b \<tturnstile> S\<^sub>b \<V>\<^sub>b ((\<Delta>\<^sub>b, Suc p'') # s\<^sub>b') \<leadsto>\<^sub>b 
+      S\<^sub>b (Lam\<^sub>b \<Delta>\<^sub>b p' # \<V>\<^sub>b) ((\<Delta>\<^sub>b, p'') # s\<^sub>b')" by simp
+    ultimately have "iter (\<tturnstile> \<C>\<^sub>b \<leadsto>\<^sub>b) (S\<^sub>b \<V>\<^sub>b ((\<Delta>\<^sub>b, Suc (Suc p'')) # s\<^sub>b')) 
+      (S\<^sub>b (Lam\<^sub>b \<Delta>\<^sub>b p' # \<V>\<^sub>b) ((\<Delta>\<^sub>b, p'') # s\<^sub>b'))" by (metis iter_step iter_refl)
+    with B S False P show ?thesis by auto
+  qed
 next
   case (ev\<^sub>e_apply v\<^sub>e \<Delta>\<^sub>e' \<C>\<^sub>e' n \<V>\<^sub>e \<Delta>\<^sub>e \<C>\<^sub>e s\<^sub>e)
   then obtain \<V>\<^sub>b s\<^sub>b where B: "\<Sigma>\<^sub>b = S\<^sub>b \<V>\<^sub>b s\<^sub>b \<and> v\<^sub>e # Lam\<^sub>e \<Delta>\<^sub>e' \<C>\<^sub>e' n # \<V>\<^sub>e = unflatten_values \<C>\<^sub>b \<V>\<^sub>b \<and> 
-    (\<Delta>\<^sub>e, Apply\<^sub>e # \<C>\<^sub>e) # s\<^sub>e = unflatten_stack \<C>\<^sub>b s\<^sub>b" by fastforce
-  with ev\<^sub>e_apply have "orderly_code \<C>\<^sub>b 0 \<and> orderly_stack s\<^sub>b (length \<C>\<^sub>b)" by simp
-  with B obtain \<Delta>\<^sub>b p s\<^sub>b' where S: "s\<^sub>b = (\<Delta>\<^sub>b, Suc p) # s\<^sub>b' \<and> 
-    \<Delta>\<^sub>e = map (unflatten_values \<C>\<^sub>b) \<Delta>\<^sub>b \<and> lookup \<C>\<^sub>b p = Some Apply\<^sub>b \<and> \<C>\<^sub>e = unflatten_code \<C>\<^sub>b p \<and> 
-      s\<^sub>e = unflatten_stack \<C>\<^sub>b s\<^sub>b'" by (metis unflatten_stack_to_apply)
-  from B obtain v\<^sub>b \<Delta>\<^sub>b' p' \<V>\<^sub>b' where V: "\<V>\<^sub>b = v\<^sub>b # Lam\<^sub>b \<Delta>\<^sub>b' p' n # \<V>\<^sub>b' \<and> 
+    (\<Delta>\<^sub>e, Apply\<^sub>e # \<C>\<^sub>e) # s\<^sub>e = unflatten_stack \<C>\<^sub>b s\<^sub>b" by force
+  with ev\<^sub>e_apply have "orderly_code \<C>\<^sub>b 0 \<and> orderly_stack s\<^sub>b (length \<C>\<^sub>b) \<and> block_structured\<^sub>b \<C>\<^sub>b" 
+    by simp
+  with B obtain \<Delta>\<^sub>b p s\<^sub>b' where S: "s\<^sub>b = (\<Delta>\<^sub>b, Suc p) # s\<^sub>b' \<and> \<Delta>\<^sub>e = map (unflatten_values \<C>\<^sub>b) \<Delta>\<^sub>b \<and> 
+      ((lookup \<C>\<^sub>b p = Some Apply\<^sub>b \<and> \<C>\<^sub>e = unflatten_code \<C>\<^sub>b p) \<or>
+      (\<exists>p' n. p = Suc p' \<and> lookup \<C>\<^sub>b (Suc p') = Some (Alloc\<^sub>b n) \<and> lookup \<C>\<^sub>b p' = Some Apply\<^sub>b \<and> 
+        \<C>\<^sub>e = unflatten_code \<C>\<^sub>b p')) \<and> s\<^sub>e = unflatten_stack \<C>\<^sub>b s\<^sub>b'" 
+    by (metis unflatten_stack_to_apply)
+  from B obtain v\<^sub>b \<Delta>\<^sub>b' p' \<V>\<^sub>b' where V: "\<V>\<^sub>b = v\<^sub>b # Lam\<^sub>b \<Delta>\<^sub>b' p' # \<V>\<^sub>b' \<and> 
     v\<^sub>e = unflatten_closure \<C>\<^sub>b v\<^sub>b \<and> \<Delta>\<^sub>e' = map (unflatten_values \<C>\<^sub>b) \<Delta>\<^sub>b' \<and> 
-      \<C>\<^sub>e' = unflatten_code \<C>\<^sub>b p' \<and> \<V>\<^sub>e = unflatten_values \<C>\<^sub>b \<V>\<^sub>b'" by fastforce
-  from S have "\<C>\<^sub>b \<tturnstile> S\<^sub>b (v\<^sub>b # Lam\<^sub>b \<Delta>\<^sub>b' p' n # \<V>\<^sub>b') ((\<Delta>\<^sub>b, Suc p) # s\<^sub>b') \<leadsto>\<^sub>b
-    S\<^sub>b \<V>\<^sub>b' (([v\<^sub>b] # \<Delta>\<^sub>b', p') # (\<Delta>\<^sub>b, p) # s\<^sub>b')" by simp
-  hence "iter (\<tturnstile> \<C>\<^sub>b \<leadsto>\<^sub>b) (S\<^sub>b (v\<^sub>b # Lam\<^sub>b \<Delta>\<^sub>b' p' n # \<V>\<^sub>b') ((\<Delta>\<^sub>b, Suc p) # s\<^sub>b')) 
-    (S\<^sub>b \<V>\<^sub>b' (([v\<^sub>b] # \<Delta>\<^sub>b', p') # (\<Delta>\<^sub>b, p) # s\<^sub>b'))" by simp
-  with B S V show ?case by auto       
+      \<C>\<^sub>e' = unflatten_code \<C>\<^sub>b p' \<and> n = alloc_size \<C>\<^sub>b p' \<and> \<V>\<^sub>e = unflatten_values \<C>\<^sub>b \<V>\<^sub>b'" by fastforce
+  show ?case
+  proof (cases "lookup \<C>\<^sub>b p = Some Apply\<^sub>b \<and> \<C>\<^sub>e = unflatten_code \<C>\<^sub>b p")
+    case True
+    with S have "\<C>\<^sub>b \<tturnstile> S\<^sub>b (v\<^sub>b # Lam\<^sub>b \<Delta>\<^sub>b' p' # \<V>\<^sub>b') ((\<Delta>\<^sub>b, Suc p) # s\<^sub>b') \<leadsto>\<^sub>b
+      S\<^sub>b \<V>\<^sub>b' (([v\<^sub>b] # \<Delta>\<^sub>b', p') # (\<Delta>\<^sub>b, p) # s\<^sub>b')" by simp
+    hence "iter (\<tturnstile> \<C>\<^sub>b \<leadsto>\<^sub>b) (S\<^sub>b (v\<^sub>b # Lam\<^sub>b \<Delta>\<^sub>b' p' # \<V>\<^sub>b') ((\<Delta>\<^sub>b, Suc p) # s\<^sub>b')) 
+      (S\<^sub>b \<V>\<^sub>b' (([v\<^sub>b] # \<Delta>\<^sub>b', p') # (\<Delta>\<^sub>b, p) # s\<^sub>b'))" by simp
+    with B S V True show ?thesis by fastforce
+  next
+    case False
+    with S obtain p'' m where P: "p = Suc p'' \<and> lookup \<C>\<^sub>b (Suc p'') = Some (Alloc\<^sub>b m) \<and> 
+      lookup \<C>\<^sub>b p'' = Some Apply\<^sub>b \<and> \<C>\<^sub>e = unflatten_code \<C>\<^sub>b p''" by blast
+    with S have "\<C>\<^sub>b \<tturnstile> S\<^sub>b (v\<^sub>b # Lam\<^sub>b \<Delta>\<^sub>b' p' # \<V>\<^sub>b') ((\<Delta>\<^sub>b, Suc (Suc p'')) # s\<^sub>b') \<leadsto>\<^sub>b 
+      S\<^sub>b (v\<^sub>b # Lam\<^sub>b \<Delta>\<^sub>b' p' # \<V>\<^sub>b') ((\<Delta>\<^sub>b, Suc p'') # s\<^sub>b')" by simp
+    moreover from S P have "\<C>\<^sub>b \<tturnstile> S\<^sub>b (v\<^sub>b # Lam\<^sub>b \<Delta>\<^sub>b' p' # \<V>\<^sub>b') ((\<Delta>\<^sub>b, Suc p'') # s\<^sub>b') \<leadsto>\<^sub>b 
+      S\<^sub>b \<V>\<^sub>b' (([v\<^sub>b] # \<Delta>\<^sub>b', p') # (\<Delta>\<^sub>b, p'') # s\<^sub>b')" by simp
+    ultimately have "iter (\<tturnstile> \<C>\<^sub>b \<leadsto>\<^sub>b) (S\<^sub>b (v\<^sub>b # Lam\<^sub>b \<Delta>\<^sub>b' p' # \<V>\<^sub>b') ((\<Delta>\<^sub>b, Suc (Suc p'')) # s\<^sub>b')) 
+      (S\<^sub>b \<V>\<^sub>b' (([v\<^sub>b] # \<Delta>\<^sub>b', p') # (\<Delta>\<^sub>b, p'') # s\<^sub>b'))" by (metis iter_step iter_refl)
+    with B S V False P show ?thesis by fastforce
+  qed
 next
   case (ev\<^sub>e_pushenv v\<^sub>e \<V>\<^sub>e \<Delta>\<^sub>e \<C>\<^sub>e s\<^sub>e)
   then obtain \<V>\<^sub>b s\<^sub>b where B: "\<Sigma>\<^sub>b = S\<^sub>b \<V>\<^sub>b s\<^sub>b \<and> v\<^sub>e # \<V>\<^sub>e = unflatten_values \<C>\<^sub>b \<V>\<^sub>b \<and> 
     ((\<Delta>\<^sub>e, PushEnv\<^sub>e # \<C>\<^sub>e) # s\<^sub>e) = unflatten_stack \<C>\<^sub>b s\<^sub>b" by fastforce
-  with ev\<^sub>e_pushenv have "orderly_code \<C>\<^sub>b 0 \<and> orderly_stack s\<^sub>b (length \<C>\<^sub>b)" by simp
-  with B obtain \<Delta>\<^sub>b p s\<^sub>b' where E: "s\<^sub>b = (\<Delta>\<^sub>b, Suc p) # s\<^sub>b' \<and> 
-    \<Delta>\<^sub>e = map (unflatten_values \<C>\<^sub>b) \<Delta>\<^sub>b \<and> lookup \<C>\<^sub>b p = Some PushEnv\<^sub>b \<and> \<C>\<^sub>e = unflatten_code \<C>\<^sub>b p \<and> 
-      s\<^sub>e = unflatten_stack \<C>\<^sub>b s\<^sub>b'" by (metis unflatten_stack_to_pushenv)
+  with ev\<^sub>e_pushenv have "orderly_code \<C>\<^sub>b 0 \<and> orderly_stack s\<^sub>b (length \<C>\<^sub>b) \<and> block_structured\<^sub>b \<C>\<^sub>b" 
+    by simp
+  with B obtain \<Delta>\<^sub>b p s\<^sub>b' where S: "s\<^sub>b = (\<Delta>\<^sub>b, Suc p) # s\<^sub>b' \<and> \<Delta>\<^sub>e = map (unflatten_values \<C>\<^sub>b) \<Delta>\<^sub>b \<and> 
+      ((lookup \<C>\<^sub>b p = Some PushEnv\<^sub>b \<and> \<C>\<^sub>e = unflatten_code \<C>\<^sub>b p) \<or>
+      (\<exists>p' n. p = Suc p' \<and> lookup \<C>\<^sub>b (Suc p') = Some (Alloc\<^sub>b n) \<and> lookup \<C>\<^sub>b p' = Some PushEnv\<^sub>b \<and> 
+        \<C>\<^sub>e = unflatten_code \<C>\<^sub>b p')) \<and> s\<^sub>e = unflatten_stack \<C>\<^sub>b s\<^sub>b'" 
+    by (metis unflatten_stack_to_pushenv)
   from B obtain v\<^sub>b \<V>\<^sub>b' where V: "\<V>\<^sub>b = v\<^sub>b # \<V>\<^sub>b' \<and> v\<^sub>e = unflatten_closure \<C>\<^sub>b v\<^sub>b \<and> 
     \<V>\<^sub>e = unflatten_values \<C>\<^sub>b \<V>\<^sub>b'" by fastforce
-  from E have "\<C>\<^sub>b \<tturnstile> S\<^sub>b (v\<^sub>b # \<V>\<^sub>b') ((\<Delta>\<^sub>b, Suc p) # s\<^sub>b') \<leadsto>\<^sub>b S\<^sub>b \<V>\<^sub>b' ((snoc_fst v\<^sub>b \<Delta>\<^sub>b, p) # s\<^sub>b')" by simp
-  hence "iter (\<tturnstile> \<C>\<^sub>b \<leadsto>\<^sub>b) (S\<^sub>b (v\<^sub>b # \<V>\<^sub>b') ((\<Delta>\<^sub>b, Suc p) # s\<^sub>b')) (S\<^sub>b \<V>\<^sub>b' ((snoc_fst v\<^sub>b \<Delta>\<^sub>b, p) # s\<^sub>b'))" 
-    by simp
-  with B E V show ?case by auto
+  show ?case
+  proof (cases "lookup \<C>\<^sub>b p = Some PushEnv\<^sub>b \<and> \<C>\<^sub>e = unflatten_code \<C>\<^sub>b p")
+    case True
+    with S have "\<C>\<^sub>b \<tturnstile> S\<^sub>b (v\<^sub>b # \<V>\<^sub>b') ((\<Delta>\<^sub>b, Suc p) # s\<^sub>b') \<leadsto>\<^sub>b S\<^sub>b \<V>\<^sub>b' ((snoc_fst v\<^sub>b \<Delta>\<^sub>b, p) # s\<^sub>b')" 
+      by simp
+    hence "iter (\<tturnstile> \<C>\<^sub>b \<leadsto>\<^sub>b) (S\<^sub>b (v\<^sub>b # \<V>\<^sub>b') ((\<Delta>\<^sub>b, Suc p) # s\<^sub>b')) (S\<^sub>b \<V>\<^sub>b' ((snoc_fst v\<^sub>b \<Delta>\<^sub>b, p) # s\<^sub>b'))" 
+      by simp
+    with B S V True show ?thesis by fastforce
+  next
+    case False
+    with S obtain p'' m where P: "p = Suc p'' \<and> lookup \<C>\<^sub>b (Suc p'') = Some (Alloc\<^sub>b m) \<and> 
+      lookup \<C>\<^sub>b p'' = Some PushEnv\<^sub>b \<and> \<C>\<^sub>e = unflatten_code \<C>\<^sub>b p''" by blast
+    with S have "\<C>\<^sub>b \<tturnstile> S\<^sub>b (v\<^sub>b # \<V>\<^sub>b') ((\<Delta>\<^sub>b, Suc (Suc p'')) # s\<^sub>b') \<leadsto>\<^sub>b 
+      S\<^sub>b (v\<^sub>b # \<V>\<^sub>b') ((\<Delta>\<^sub>b, Suc p'') # s\<^sub>b')" by simp
+    moreover from S P have "\<C>\<^sub>b \<tturnstile> S\<^sub>b (v\<^sub>b # \<V>\<^sub>b') ((\<Delta>\<^sub>b, Suc p'') # s\<^sub>b') \<leadsto>\<^sub>b 
+      S\<^sub>b \<V>\<^sub>b' ((snoc_fst v\<^sub>b \<Delta>\<^sub>b, p'') # s\<^sub>b')" by simp
+    ultimately have "iter (\<tturnstile> \<C>\<^sub>b \<leadsto>\<^sub>b) (S\<^sub>b (v\<^sub>b # \<V>\<^sub>b') ((\<Delta>\<^sub>b, Suc (Suc p'')) # s\<^sub>b')) 
+      (S\<^sub>b \<V>\<^sub>b' ((snoc_fst v\<^sub>b \<Delta>\<^sub>b, p'') # s\<^sub>b'))" by (metis iter_step iter_refl)
+    with B S V False P show ?thesis by fastforce
+  qed
 next
   case (ev\<^sub>e_return \<V>\<^sub>e \<Delta>\<^sub>e \<C>\<^sub>e s\<^sub>e)
   then obtain \<V>\<^sub>b s\<^sub>b where B: "\<Sigma>\<^sub>b = S\<^sub>b \<V>\<^sub>b s\<^sub>b \<and> \<V>\<^sub>e = unflatten_values \<C>\<^sub>b \<V>\<^sub>b \<and> 
     (\<Delta>\<^sub>e, Return\<^sub>e # \<C>\<^sub>e) # s\<^sub>e = unflatten_stack \<C>\<^sub>b s\<^sub>b" by fastforce
-  with ev\<^sub>e_return have "orderly_code \<C>\<^sub>b 0 \<and> orderly_stack s\<^sub>b (length \<C>\<^sub>b)" by simp
-  with B obtain \<Delta>\<^sub>b p s\<^sub>b' where S: "s\<^sub>b = (\<Delta>\<^sub>b, Suc p) # s\<^sub>b' \<and> 
-    \<Delta>\<^sub>e = map (unflatten_values \<C>\<^sub>b) \<Delta>\<^sub>b \<and> lookup \<C>\<^sub>b p = Some Return\<^sub>b \<and> s\<^sub>e = unflatten_stack \<C>\<^sub>b s\<^sub>b'" 
-      by (metis unflatten_stack_to_return)
-  with S have "\<C>\<^sub>b \<tturnstile> S\<^sub>b \<V>\<^sub>b ((\<Delta>\<^sub>b, Suc p) # s\<^sub>b') \<leadsto>\<^sub>b S\<^sub>b \<V>\<^sub>b s\<^sub>b'" by simp
-  hence "iter (\<tturnstile> \<C>\<^sub>b \<leadsto>\<^sub>b) (S\<^sub>b \<V>\<^sub>b ((\<Delta>\<^sub>b, Suc p) # s\<^sub>b')) (S\<^sub>b \<V>\<^sub>b s\<^sub>b')" by simp
-  with B S show ?case by fastforce
+  with ev\<^sub>e_return have "orderly_code \<C>\<^sub>b 0 \<and> orderly_stack s\<^sub>b (length \<C>\<^sub>b) \<and> block_structured\<^sub>b \<C>\<^sub>b" 
+    by simp
+  with B obtain \<Delta>\<^sub>b p s\<^sub>b' where S: "s\<^sub>b = (\<Delta>\<^sub>b, Suc p) # s\<^sub>b' \<and> \<Delta>\<^sub>e = map (unflatten_values \<C>\<^sub>b) \<Delta>\<^sub>b \<and> 
+      (lookup \<C>\<^sub>b p = Some Return\<^sub>b \<or> 
+      (\<exists>p' n. p = Suc p' \<and> lookup \<C>\<^sub>b (Suc p') = Some (Alloc\<^sub>b n) \<and> lookup \<C>\<^sub>b p' = Some Return\<^sub>b)) \<and> 
+        \<C>\<^sub>e = [] \<and> s\<^sub>e = unflatten_stack \<C>\<^sub>b s\<^sub>b'" 
+    by (metis unflatten_stack_to_return)
+  show ?case
+  proof (cases "lookup \<C>\<^sub>b p = Some Return\<^sub>b")
+    case True
+    with S have "\<C>\<^sub>b \<tturnstile> S\<^sub>b \<V>\<^sub>b ((\<Delta>\<^sub>b, Suc p) # s\<^sub>b') \<leadsto>\<^sub>b S\<^sub>b \<V>\<^sub>b s\<^sub>b'" by simp
+    hence "iter (\<tturnstile> \<C>\<^sub>b \<leadsto>\<^sub>b) (S\<^sub>b \<V>\<^sub>b ((\<Delta>\<^sub>b, Suc p) # s\<^sub>b')) (S\<^sub>b \<V>\<^sub>b s\<^sub>b')" by simp
+    with B S True show ?thesis by fastforce
+  next
+    case False
+    with S obtain p' n where P: "p = Suc p' \<and> lookup \<C>\<^sub>b (Suc p') = Some (Alloc\<^sub>b n) \<and> 
+      lookup \<C>\<^sub>b p' = Some Return\<^sub>b" by blast
+    with S have "\<C>\<^sub>b \<tturnstile> S\<^sub>b \<V>\<^sub>b ((\<Delta>\<^sub>b, Suc (Suc p')) # s\<^sub>b') \<leadsto>\<^sub>b S\<^sub>b \<V>\<^sub>b ((\<Delta>\<^sub>b, Suc p') # s\<^sub>b')" by simp
+    moreover from S P have "\<C>\<^sub>b \<tturnstile> S\<^sub>b \<V>\<^sub>b ((\<Delta>\<^sub>b, Suc p') # s\<^sub>b') \<leadsto>\<^sub>b S\<^sub>b \<V>\<^sub>b s\<^sub>b'" by simp
+    ultimately have "iter (\<tturnstile> \<C>\<^sub>b \<leadsto>\<^sub>b) (S\<^sub>b \<V>\<^sub>b ((\<Delta>\<^sub>b, Suc (Suc p')) # s\<^sub>b')) (S\<^sub>b \<V>\<^sub>b s\<^sub>b')" 
+      by (metis iter_step iter_refl)
+    with B S False P show ?thesis by fastforce
+  qed
 next
   case (ev\<^sub>e_jump v \<Delta>\<^sub>e' \<C>\<^sub>e' n \<V>\<^sub>e \<Delta>\<^sub>e \<C>\<^sub>e s\<^sub>e)
   then obtain \<V>\<^sub>b s\<^sub>b where B: "\<Sigma>\<^sub>b = S\<^sub>b \<V>\<^sub>b s\<^sub>b \<and> 
     v # Lam\<^sub>e \<Delta>\<^sub>e' \<C>\<^sub>e' n # \<V>\<^sub>e = unflatten_values \<C>\<^sub>b \<V>\<^sub>b \<and> 
-      (\<Delta>\<^sub>e, Jump\<^sub>e # \<C>\<^sub>e) # s\<^sub>e = unflatten_stack \<C>\<^sub>b s\<^sub>b" by fastforce
-  with ev\<^sub>e_jump have "orderly_code \<C>\<^sub>b 0 \<and> orderly_stack s\<^sub>b (length \<C>\<^sub>b)" by simp
-  with B obtain \<Delta>\<^sub>b p s\<^sub>b' where S: "s\<^sub>b = (\<Delta>\<^sub>b, Suc p) # s\<^sub>b' \<and> 
-    \<Delta>\<^sub>e = map (unflatten_values \<C>\<^sub>b) \<Delta>\<^sub>b \<and> lookup \<C>\<^sub>b p = Some Jump\<^sub>b \<and> s\<^sub>e = unflatten_stack \<C>\<^sub>b s\<^sub>b'" 
-      by (metis unflatten_stack_to_jump)
-  from B obtain vb \<Delta>\<^sub>b' p' \<V>\<^sub>b' where V: "\<V>\<^sub>b = vb # Lam\<^sub>b \<Delta>\<^sub>b' p' n # \<V>\<^sub>b' \<and> 
-    v = unflatten_closure \<C>\<^sub>b vb \<and> \<Delta>\<^sub>e' = map (unflatten_values \<C>\<^sub>b) \<Delta>\<^sub>b' \<and> \<C>\<^sub>e' = unflatten_code \<C>\<^sub>b p' \<and>
-      \<V>\<^sub>e = unflatten_values \<C>\<^sub>b \<V>\<^sub>b'" by fastforce
-  from S have "\<C>\<^sub>b \<tturnstile> S\<^sub>b (vb # Lam\<^sub>b \<Delta>\<^sub>b' p' n # \<V>\<^sub>b') ((\<Delta>\<^sub>b, Suc p) # s\<^sub>b') \<leadsto>\<^sub>b
-    S\<^sub>b \<V>\<^sub>b' (([vb] # \<Delta>\<^sub>b', p') # s\<^sub>b')" by simp
-  hence "iter (\<tturnstile> \<C>\<^sub>b \<leadsto>\<^sub>b) (S\<^sub>b (vb # Lam\<^sub>b \<Delta>\<^sub>b' p' n # \<V>\<^sub>b') ((\<Delta>\<^sub>b, Suc p) # s\<^sub>b')) 
-    (S\<^sub>b \<V>\<^sub>b' (([vb] # \<Delta>\<^sub>b', p') # s\<^sub>b'))" by simp
-  with B S V show ?case by auto                                              
+      (\<Delta>\<^sub>e, Jump\<^sub>e # \<C>\<^sub>e) # s\<^sub>e = unflatten_stack \<C>\<^sub>b s\<^sub>b" by force
+  with ev\<^sub>e_jump have "orderly_code \<C>\<^sub>b 0 \<and> orderly_stack s\<^sub>b (length \<C>\<^sub>b) \<and> block_structured\<^sub>b \<C>\<^sub>b" 
+    by simp
+  with B obtain \<Delta>\<^sub>b p s\<^sub>b' where S: "s\<^sub>b = (\<Delta>\<^sub>b, Suc p) # s\<^sub>b' \<and> \<Delta>\<^sub>e = map (unflatten_values \<C>\<^sub>b) \<Delta>\<^sub>b \<and> 
+    (lookup \<C>\<^sub>b p = Some Jump\<^sub>b \<or> (\<exists>p' n. p = Suc p' \<and> lookup \<C>\<^sub>b (Suc p') = Some (Alloc\<^sub>b n) \<and> 
+      lookup \<C>\<^sub>b p' = Some Jump\<^sub>b)) \<and> \<C>\<^sub>e = [] \<and> s\<^sub>e = unflatten_stack \<C>\<^sub>b s\<^sub>b'" 
+    by (metis unflatten_stack_to_jump)
+  from B obtain v\<^sub>b \<Delta>\<^sub>b' p' \<V>\<^sub>b' where V: "\<V>\<^sub>b = v\<^sub>b # Lam\<^sub>b \<Delta>\<^sub>b' p' # \<V>\<^sub>b' \<and> 
+    v = unflatten_closure \<C>\<^sub>b v\<^sub>b \<and> \<Delta>\<^sub>e' = map (unflatten_values \<C>\<^sub>b) \<Delta>\<^sub>b' \<and> \<C>\<^sub>e' = unflatten_code \<C>\<^sub>b p' \<and>
+      n = alloc_size \<C>\<^sub>b p' \<and> \<V>\<^sub>e = unflatten_values \<C>\<^sub>b \<V>\<^sub>b'" by fastforce
+  show ?case
+  proof (cases "lookup \<C>\<^sub>b p = Some Jump\<^sub>b")
+    case True
+    with S have "\<C>\<^sub>b \<tturnstile> S\<^sub>b (v\<^sub>b # Lam\<^sub>b \<Delta>\<^sub>b' p' # \<V>\<^sub>b') ((\<Delta>\<^sub>b, Suc p) # s\<^sub>b') \<leadsto>\<^sub>b
+      S\<^sub>b \<V>\<^sub>b' (([v\<^sub>b] # \<Delta>\<^sub>b', p') # s\<^sub>b')" by simp
+    hence "iter (\<tturnstile> \<C>\<^sub>b \<leadsto>\<^sub>b) (S\<^sub>b (v\<^sub>b # Lam\<^sub>b \<Delta>\<^sub>b' p' # \<V>\<^sub>b') ((\<Delta>\<^sub>b, Suc p) # s\<^sub>b')) 
+      (S\<^sub>b \<V>\<^sub>b' (([v\<^sub>b] # \<Delta>\<^sub>b', p') # s\<^sub>b'))" by simp
+    with B S V True show ?thesis by fastforce
+  next
+    case False
+    with S obtain p'' m where P: "p = Suc p'' \<and> lookup \<C>\<^sub>b (Suc p'') = Some (Alloc\<^sub>b m) \<and> 
+      lookup \<C>\<^sub>b p'' = Some Jump\<^sub>b" by blast
+    with S have "\<C>\<^sub>b \<tturnstile> S\<^sub>b (v\<^sub>b # Lam\<^sub>b \<Delta>\<^sub>b' p' # \<V>\<^sub>b') ((\<Delta>\<^sub>b, Suc (Suc p'')) # s\<^sub>b') \<leadsto>\<^sub>b 
+      S\<^sub>b (v\<^sub>b # Lam\<^sub>b \<Delta>\<^sub>b' p' # \<V>\<^sub>b') ((\<Delta>\<^sub>b, Suc p'') # s\<^sub>b')" by simp
+    moreover from S P have "\<C>\<^sub>b \<tturnstile> S\<^sub>b (v\<^sub>b # Lam\<^sub>b \<Delta>\<^sub>b' p' # \<V>\<^sub>b') ((\<Delta>\<^sub>b, Suc p'') # s\<^sub>b') \<leadsto>\<^sub>b 
+      S\<^sub>b \<V>\<^sub>b' (([v\<^sub>b] # \<Delta>\<^sub>b', p') # s\<^sub>b')" by simp
+    ultimately have "iter (\<tturnstile> \<C>\<^sub>b \<leadsto>\<^sub>b) (S\<^sub>b (v\<^sub>b # Lam\<^sub>b \<Delta>\<^sub>b' p' # \<V>\<^sub>b') ((\<Delta>\<^sub>b, Suc (Suc p'')) # s\<^sub>b')) 
+      (S\<^sub>b \<V>\<^sub>b' (([v\<^sub>b] # \<Delta>\<^sub>b', p') # s\<^sub>b'))" by (metis iter_step iter_refl)
+    with B S V False P show ?thesis by fastforce
+  qed
 qed
 
 lemma iter_correct\<^sub>b [simp]: "iter (\<leadsto>\<^sub>e) (unflatten_state \<C>\<^sub>b \<Sigma>\<^sub>b) \<Sigma>\<^sub>e' \<Longrightarrow> orderly_state \<C>\<^sub>b \<Sigma>\<^sub>b \<Longrightarrow>
